theories/reactive/utp_rea_core.thy
@@ -1,0 +1,201 @@
+section \<open> Reactive Processes Core Definitions \<close>
+
+theory utp_rea_core
+imports
+  "UTP-Toolkit.Trace_Algebra"
+  "UTP.utp_concurrency"
+  "UTP-Designs.utp_designs"
+begin recall_syntax
+
+subsection \<open> Alphabet and Signature \<close>
+
+text \<open> The alphabet of reactive processes contains a boolean variable $wait$, which denotes whether
+  a process is exhibiting an intermediate observation. It also has the variable $tr$ which denotes
+  the trace history of a process. The type parameter @{typ "'t"} represents the trace model being
+  used, which must form a trace algebra~\cite{Foster17b}, and thus provides the theory of ``generalised 
+  reactive processes''~\cite{Foster17b}. The reactive process alphabet also extends
+  the design alphabet, and thus includes the $ok$ variable. For more information on these, see
+  the UTP book~\cite{Hoare&98}, or the associated tutorial~\cite{Cavalcanti&06}. \<close>
+
+alphabet 't::trace rp_vars = des_vars +
+  wait :: bool
+  tr   :: "'t"
+
+type_synonym ('t, '\<alpha>) rp = "('t, '\<alpha>) rp_vars_scheme des"
+
+type_synonym ('t,'\<alpha>,'\<beta>) rel_rp  = "(('t,'\<alpha>) rp, ('t,'\<beta>) rp) urel"
+type_synonym ('t,'\<alpha>) hrel_rp  = "('t,'\<alpha>) rp hrel"
+
+translations
+  (type) "('t,'\<alpha>) rp" <= (type) "('t, '\<alpha>) rp_vars_scheme des"
+  (type) "('t,'\<alpha>) rp" <= (type) "('t, '\<alpha>) rp_vars_ext des"
+  (type) "('t,'\<alpha>,'\<beta>) rel_rp" <= (type) "(('t,'\<alpha>) rp, ('\<gamma>,'\<beta>) rp) urel"
+  (type) "('t, '\<alpha>) hrel_rp"  <= (type) "('t, '\<alpha>) rp hrel"
+
+text \<open> As for designs, we set up various types to represent reactive processes. The main types
+  to be used are @{typ "('t,'\<alpha>,'\<beta>) rel_rp"} and @{typ "('t,'\<alpha>) hrel_rp"}, which correspond
+  to heterogeneous/homogeneous reactive processes whose trace model is @{typ "'t"} and alphabet 
+  types are @{typ "'\<alpha>"} and @{typ "'\<beta>"}. We also set up some useful syntax translations for these. \<close>
+
+notation rp_vars_child_lens\<^sub>a ("\<Sigma>\<^sub>r")
+notation rp_vars_child_lens ("\<Sigma>\<^sub>R")
+
+syntax
+  "_svid_rea_alpha"  :: "svid" ("\<Sigma>\<^sub>R")
+
+translations
+  "_svid_rea_alpha" => "CONST rp_vars_child_lens"
+
+text \<open> Lens @{term "\<Sigma>\<^sub>R"} exists because reactive alphabets are extensible. @{term "\<Sigma>\<^sub>R"} points
+  to the portion of the alphabet / state space that is neither $ok$, $wait$, or $tr$. \<close>
+
+declare rp_vars.splits [alpha_splits]
+declare rp_vars.defs [lens_defs]
+declare zero_list_def [upred_defs]
+declare plus_list_def [upred_defs]
+declare prefixE [elim]
+  
+text \<open>
+  The two locale interpretations below are a technicality to improve automatic
+  proof support via the predicate and relational tactics. This is to enable the
+  (re-)interpretation of state spaces to remove any occurrences of lens types
+  after the proof tactics @{method pred_simp} and @{method rel_simp}, or any
+  of their derivatives have been applied. Eventually, it would be desirable to
+  automate both interpretations as part of a custom outer command for defining
+  alphabets.
+\<close>
+
+interpretation rp_vars:
+  lens_interp "\<lambda>(ok, r). (ok, wait\<^sub>v r, tr\<^sub>v r, more r)"
+  apply (unfold_locales)
+  apply (rule injI)
+  apply (clarsimp)
+  done
+
+interpretation rp_vars_rel: lens_interp "\<lambda>(ok, ok', r, r').
+  (ok, ok', wait\<^sub>v r, wait\<^sub>v r', tr\<^sub>v r, tr\<^sub>v r', more r, more r')"
+  apply (unfold_locales)
+  apply (rule injI)
+  apply (clarsimp)
+  done
+
+text \<open> The following syntactic orders exist to help to order lens names when, for example, 
+  performing substitution, to achieve normalisation of terms. \<close>
+
+lemma rea_var_ords [usubst]:
+  "$tr \<prec>\<^sub>v $tr\<acute>" "$wait \<prec>\<^sub>v $wait\<acute>"
+  "$ok \<prec>\<^sub>v $tr" "$ok\<acute> \<prec>\<^sub>v $tr\<acute>" "$ok \<prec>\<^sub>v $tr\<acute>" "$ok\<acute> \<prec>\<^sub>v $tr"
+  "$ok \<prec>\<^sub>v $wait" "$ok\<acute> \<prec>\<^sub>v $wait\<acute>" "$ok \<prec>\<^sub>v $wait\<acute>" "$ok\<acute> \<prec>\<^sub>v $wait"
+  "$tr \<prec>\<^sub>v $wait" "$tr\<acute> \<prec>\<^sub>v $wait\<acute>" "$tr \<prec>\<^sub>v $wait\<acute>" "$tr\<acute> \<prec>\<^sub>v $wait"
+  by (simp_all add: var_name_ord_def)
+
+abbreviation wait_f::"('t::trace, '\<alpha>, '\<beta>) rel_rp \<Rightarrow> ('t, '\<alpha>, '\<beta>) rel_rp"
+where "wait_f R \<equiv> R\<lbrakk>false/$wait\<rbrakk>"
+
+abbreviation wait_t::"('t::trace, '\<alpha>, '\<beta>) rel_rp \<Rightarrow> ('t, '\<alpha>, '\<beta>) rel_rp"
+where "wait_t R \<equiv> R\<lbrakk>true/$wait\<rbrakk>"
+  
+syntax
+  "_wait_f"  :: "logic \<Rightarrow> logic" ("_\<^sub>f" [1000] 1000)
+  "_wait_t"  :: "logic \<Rightarrow> logic" ("_\<^sub>t" [1000] 1000)
+
+translations
+  "P \<^sub>f" \<rightleftharpoons> "CONST usubst (CONST subst_upd CONST id (CONST ivar CONST wait) false) P"
+  "P \<^sub>t" \<rightleftharpoons> "CONST usubst (CONST subst_upd CONST id (CONST ivar CONST wait) true) P"
+
+abbreviation lift_rea :: "_ \<Rightarrow> _" ("\<lceil>_\<rceil>\<^sub>R") where
+"\<lceil>P\<rceil>\<^sub>R \<equiv> P \<oplus>\<^sub>p (\<Sigma>\<^sub>R \<times>\<^sub>L \<Sigma>\<^sub>R)"
+
+abbreviation drop_rea :: "('t::trace, '\<alpha>, '\<beta>) rel_rp \<Rightarrow> ('\<alpha>, '\<beta>) urel" ("\<lfloor>_\<rfloor>\<^sub>R") where
+"\<lfloor>P\<rfloor>\<^sub>R \<equiv> P \<restriction>\<^sub>e (\<Sigma>\<^sub>R \<times>\<^sub>L \<Sigma>\<^sub>R)"
+
+abbreviation rea_pre_lift :: "_ \<Rightarrow> _" ("\<lceil>_\<rceil>\<^sub>R\<^sub><") where "\<lceil>n\<rceil>\<^sub>R\<^sub>< \<equiv> \<lceil>\<lceil>n\<rceil>\<^sub><\<rceil>\<^sub>R"
+
+subsection \<open> Reactive Lemmas \<close>
+
+lemma unrest_ok_lift_rea [unrest]:
+  "$ok \<sharp> \<lceil>P\<rceil>\<^sub>R" "$ok\<acute> \<sharp> \<lceil>P\<rceil>\<^sub>R"
+  by (pred_auto)+
+
+lemma unrest_wait_lift_rea [unrest]:
+  "$wait \<sharp> \<lceil>P\<rceil>\<^sub>R" "$wait\<acute> \<sharp> \<lceil>P\<rceil>\<^sub>R"
+  by (pred_auto)+
+
+lemma unrest_tr_lift_rea [unrest]:
+  "$tr \<sharp> \<lceil>P\<rceil>\<^sub>R" "$tr\<acute> \<sharp> \<lceil>P\<rceil>\<^sub>R"
+  by (pred_auto)+
+
+lemma wait_tr_bij_lemma: "bij_lens (wait\<^sub>a +\<^sub>L tr\<^sub>a +\<^sub>L \<Sigma>\<^sub>r)"
+  by (unfold_locales, auto simp add: lens_defs)
+
+lemma des_lens_equiv_wait_tr_rest: "\<Sigma>\<^sub>D \<approx>\<^sub>L wait +\<^sub>L tr +\<^sub>L \<Sigma>\<^sub>R"
+proof -
+  have "wait +\<^sub>L tr +\<^sub>L \<Sigma>\<^sub>R = (wait\<^sub>a +\<^sub>L tr\<^sub>a +\<^sub>L \<Sigma>\<^sub>r) ;\<^sub>L \<Sigma>\<^sub>D"
+    by (simp add: plus_lens_distr wait_def tr_def rp_vars_child_lens_def)
+  also have "... \<approx>\<^sub>L 1\<^sub>L ;\<^sub>L \<Sigma>\<^sub>D"
+    using lens_equiv_via_bij wait_tr_bij_lemma by auto
+  also have "... = \<Sigma>\<^sub>D"
+    by (simp)
+  finally show ?thesis
+    using lens_equiv_sym by blast
+qed
+
+lemma rea_lens_bij: "bij_lens (ok +\<^sub>L wait +\<^sub>L tr +\<^sub>L \<Sigma>\<^sub>R)"
+proof -
+  have "ok +\<^sub>L wait +\<^sub>L tr +\<^sub>L \<Sigma>\<^sub>R \<approx>\<^sub>L ok +\<^sub>L \<Sigma>\<^sub>D"
+    using des_lens_equiv_wait_tr_rest des_vars_indeps lens_equiv_sym lens_plus_eq_right by blast
+  also have "... \<approx>\<^sub>L 1\<^sub>L"
+    using bij_lens_equiv_id[of "ok +\<^sub>L \<Sigma>\<^sub>D"] by (simp add: ok_des_bij_lens)
+  finally show ?thesis
+    by (simp add: bij_lens_equiv_id)
+qed
+
+lemma seqr_wait_true [usubst]: "(P ;; Q) \<^sub>t = (P \<^sub>t ;; Q)"
+  by (rel_auto)
+
+lemma seqr_wait_false [usubst]: "(P ;; Q) \<^sub>f = (P \<^sub>f ;; Q)"
+  by (rel_auto)
+
+subsection {* Trace contribution lens *}
+
+text \<open> The following lens represents the portion of the state-space that is the difference
+  between $tr'$ and $tr$, that is the contribution that a process is making to the trace
+  history. \<close>
+
+definition tcontr :: "'t::trace \<Longrightarrow> ('t, '\<alpha>) rp \<times> ('t, '\<alpha>) rp" ("tt") where
+  [lens_defs]:
+  "tcontr = \<lparr> lens_get = (\<lambda> s. get\<^bsub>($tr\<acute>)\<^sub>v\<^esub> s - get\<^bsub>($tr)\<^sub>v\<^esub> s) , 
+              lens_put = (\<lambda> s v. put\<^bsub>($tr\<acute>)\<^sub>v\<^esub> s (get\<^bsub>($tr)\<^sub>v\<^esub> s + v)) \<rparr>"
+
+definition itrace :: "'t::trace \<Longrightarrow> ('t, '\<alpha>) rp \<times> ('t, '\<alpha>) rp" ("\<^bold>i\<^bold>t") where
+  [lens_defs]:
+  "itrace = \<lparr> lens_get = get\<^bsub>($tr)\<^sub>v\<^esub>, 
+              lens_put = (\<lambda> s v. put\<^bsub>($tr\<acute>)\<^sub>v\<^esub> (put\<^bsub>($tr)\<^sub>v\<^esub> s v) v) \<rparr>"
+    
+lemma tcontr_mwb_lens [simp]: "mwb_lens tt"
+  by (unfold_locales, simp_all add: lens_defs prod.case_eq_if)
+
+lemma itrace_mwb_lens [simp]: "mwb_lens \<^bold>i\<^bold>t"
+  by (unfold_locales, simp_all add: lens_defs prod.case_eq_if)
+    
+syntax
+  "_svid_tcontr"  :: "svid" ("tt")
+  "_svid_itrace"  :: "svid" ("\<^bold>i\<^bold>t")
+
+translations
+  "_svid_tcontr" == "CONST tcontr"
+  "_svid_itrace" == "CONST itrace"
+  
+lemma tcontr_alt_def: "&tt = ($tr\<acute> - $tr)"
+  by (rel_auto)
+
+lemma tcontr_alt_def': "utp_expr.var tt = ($tr\<acute> - $tr)"
+  by (rel_auto)
+
+lemma tt_indeps [simp]:
+  assumes "x \<bowtie> ($tr)\<^sub>v" "x \<bowtie> ($tr\<acute>)\<^sub>v"
+  shows "x \<bowtie> tt" "tt \<bowtie> x"
+  using assms
+  by (unfold lens_indep_def, safe, simp_all add: tcontr_def, (metis lens_indep_get var_update_out)+)
+
+end
