theories/reactive/utp_rea_parallel.thy
@@ -1,0 +1,174 @@
+section \<open> Reactive Parallel-by-Merge \<close>
+
+theory utp_rea_parallel
+  imports utp_rea_healths
+begin
+
+text \<open> We show closure of parallel by merge under the reactive healthiness conditions by means
+  of suitable restrictions on the merge predicate. We first define healthiness conditions
+  for R1 and R2 merge predicates. \<close>
+
+definition R1m :: "('t :: trace, '\<alpha>) rp merge \<Rightarrow> ('t, '\<alpha>) rp merge"
+  where [upred_defs]: "R1m(M) = (M \<and> $tr\<^sub>< \<le>\<^sub>u $tr\<acute>)"
+
+definition R1m' :: "('t :: trace, '\<alpha>) rp merge \<Rightarrow> ('t, '\<alpha>) rp merge"
+  where [upred_defs]: "R1m'(M) = (M \<and> $tr\<^sub>< \<le>\<^sub>u $tr\<acute> \<and> $tr\<^sub>< \<le>\<^sub>u $0-tr \<and> $tr\<^sub>< \<le>\<^sub>u $1-tr)"
+
+text \<open> A merge predicate can access the history through $tr$, as usual, but also through $0.tr$ and
+  $1.tr$. Thus we have to remove the latter two histories as well to satisfy R2 for the overall
+  construction. \<close>
+
+term "M\<lbrakk>0,x,k/y,z,a\<rbrakk>"
+  
+term "M\<lbrakk>0,$tr\<acute> - $tr\<^sub><,$0-tr - $tr\<^sub><,$1-tr - $tr\<^sub></$tr\<^sub><,$tr\<acute>,$0-tr,$1-tr\<rbrakk>"
+  
+definition R2m :: "('t :: trace, '\<alpha>) rp merge \<Rightarrow> ('t, '\<alpha>) rp merge"
+  where [upred_defs]: "R2m(M) = R1m(M\<lbrakk>0,$tr\<acute> - $tr\<^sub><,$0-tr - $tr\<^sub><,$1-tr - $tr\<^sub></$tr\<^sub><,$tr\<acute>,$0-tr,$1-tr\<rbrakk>)"
+
+definition R2m' :: "('t :: trace, '\<alpha>) rp merge \<Rightarrow> ('t, '\<alpha>) rp merge"
+  where [upred_defs]: "R2m'(M) = R1m'(M\<lbrakk>0,$tr\<acute> - $tr\<^sub><,$0-tr - $tr\<^sub><,$1-tr - $tr\<^sub></$tr\<^sub><,$tr\<acute>,$0-tr,$1-tr\<rbrakk>)"
+
+definition R2cm :: "('t :: trace, '\<alpha>) rp merge \<Rightarrow> ('t, '\<alpha>) rp merge"
+  where [upred_defs]: "R2cm(M) = M\<lbrakk>0,$tr\<acute> - $tr\<^sub><,$0-tr - $tr\<^sub><,$1-tr - $tr\<^sub></$tr\<^sub><,$tr\<acute>,$0-tr,$1-tr\<rbrakk> \<triangleleft> $tr\<^sub>< \<le>\<^sub>u $tr\<acute> \<triangleright> M"
+
+lemma R2m'_form:
+  "R2m'(M) =
+  (\<^bold>\<exists> (tt\<^sub>p, tt\<^sub>0, tt\<^sub>1) \<bullet> M\<lbrakk>0,\<guillemotleft>tt\<^sub>p\<guillemotright>,\<guillemotleft>tt\<^sub>0\<guillemotright>,\<guillemotleft>tt\<^sub>1\<guillemotright>/$tr\<^sub><,$tr\<acute>,$0-tr,$1-tr\<rbrakk>
+                    \<and> $tr\<acute> =\<^sub>u $tr\<^sub>< + \<guillemotleft>tt\<^sub>p\<guillemotright>
+                    \<and> $0-tr =\<^sub>u $tr\<^sub>< + \<guillemotleft>tt\<^sub>0\<guillemotright>
+                    \<and> $1-tr =\<^sub>u $tr\<^sub>< + \<guillemotleft>tt\<^sub>1\<guillemotright>)"
+  by (rel_auto, metis diff_add_cancel_left')
+
+lemma R1m_idem: "R1m(R1m(P)) = R1m(P)"
+  by (rel_auto)
+
+lemma R1m_seq_lemma: "R1m(R1m(M) ;; R1(P)) = R1m(M) ;; R1(P)"
+  by (rel_auto)
+
+lemma R1m_seq [closure]:
+  assumes "M is R1m" "P is R1"
+  shows "M ;; P is R1m"
+proof -
+  from assms have "R1m(M ;; P) = R1m(R1m(M) ;; R1(P))"
+    by (simp add: Healthy_if)
+  also have "... = R1m(M) ;; R1(P)"
+    by (simp add: R1m_seq_lemma)
+  also have "... = M ;; P"
+    by (simp add: Healthy_if assms)
+  finally show ?thesis
+    by (simp add: Healthy_def)
+qed
+
+lemma R2m_idem: "R2m(R2m(P)) = R2m(P)"
+  by (rel_auto)
+
+lemma R2m_seq_lemma: "R2m'(R2m'(M) ;; R2(P)) = R2m'(M) ;; R2(P)"
+  apply (simp add: R2m'_form R2_form)
+  apply (rel_auto)
+  apply (metis (no_types, lifting) add.assoc)+
+done
+
+lemma R2m'_seq [closure]:
+  assumes "M is R2m'" "P is R2"
+  shows "M ;; P is R2m'"
+  by (metis Healthy_def' R2m_seq_lemma assms(1) assms(2))
+
+lemma R1_par_by_merge [closure]:
+  "M is R1m \<Longrightarrow> (P \<parallel>\<^bsub>M\<^esub> Q) is R1"
+  by (rel_blast)
+    
+lemma R2_R2m'_pbm: "R2(P \<parallel>\<^bsub>M\<^esub> Q) = (R2(P) \<parallel>\<^bsub>R2m'(M)\<^esub> R2(Q))"
+proof -
+  have "(R2(P) \<parallel>\<^bsub>R2m'(M)\<^esub> R2(Q)) = ((R2(P) \<parallel>\<^sub>s R2(Q)) ;;
+                   (\<^bold>\<exists> (tt\<^sub>p, tt\<^sub>0, tt\<^sub>1) \<bullet> M\<lbrakk>0,\<guillemotleft>tt\<^sub>p\<guillemotright>,\<guillemotleft>tt\<^sub>0\<guillemotright>,\<guillemotleft>tt\<^sub>1\<guillemotright>/$tr\<^sub><,$tr\<acute>,$0-tr,$1-tr\<rbrakk>
+                                     \<and> $tr\<acute> =\<^sub>u $tr\<^sub>< + \<guillemotleft>tt\<^sub>p\<guillemotright>
+                                     \<and> $0-tr =\<^sub>u $tr\<^sub>< + \<guillemotleft>tt\<^sub>0\<guillemotright>
+                                     \<and> $1-tr =\<^sub>u $tr\<^sub>< + \<guillemotleft>tt\<^sub>1\<guillemotright>))"
+    by (simp add: par_by_merge_def R2m'_form)
+  also have "... = (\<^bold>\<exists> (tt\<^sub>p, tt\<^sub>0, tt\<^sub>1) \<bullet> ((R2(P) \<parallel>\<^sub>s R2(Q)) ;; (M\<lbrakk>0,\<guillemotleft>tt\<^sub>p\<guillemotright>,\<guillemotleft>tt\<^sub>0\<guillemotright>,\<guillemotleft>tt\<^sub>1\<guillemotright>/$tr\<^sub><,$tr\<acute>,$0-tr,$1-tr\<rbrakk>
+                                                  \<and> $tr\<acute> =\<^sub>u $tr\<^sub>< + \<guillemotleft>tt\<^sub>p\<guillemotright>
+                                                  \<and> $0-tr =\<^sub>u $tr\<^sub>< + \<guillemotleft>tt\<^sub>0\<guillemotright>
+                                                  \<and> $1-tr =\<^sub>u $tr\<^sub>< + \<guillemotleft>tt\<^sub>1\<guillemotright>)))"
+    by (rel_blast)
+  also have "... = (\<^bold>\<exists> (tt\<^sub>p, tt\<^sub>0, tt\<^sub>1) \<bullet> (((R2(P) \<parallel>\<^sub>s R2(Q)) \<and> $0-tr\<acute> =\<^sub>u $tr\<^sub><\<acute> + \<guillemotleft>tt\<^sub>0\<guillemotright> \<and> $1-tr\<acute> =\<^sub>u $tr\<^sub><\<acute> + \<guillemotleft>tt\<^sub>1\<guillemotright>) ;;
+                                      (M\<lbrakk>0,\<guillemotleft>tt\<^sub>p\<guillemotright>,\<guillemotleft>tt\<^sub>0\<guillemotright>,\<guillemotleft>tt\<^sub>1\<guillemotright>/$tr\<^sub><,$tr\<acute>,$0-tr,$1-tr\<rbrakk> \<and> $tr\<acute> =\<^sub>u $tr\<^sub>< + \<guillemotleft>tt\<^sub>p\<guillemotright>)))"
+    by (rel_blast)
+  also have "... = (\<^bold>\<exists> (tt\<^sub>p, tt\<^sub>0, tt\<^sub>1) \<bullet> (((R2(P) \<parallel>\<^sub>s R2(Q)) \<and> $0-tr\<acute> =\<^sub>u $tr\<^sub><\<acute> + \<guillemotleft>tt\<^sub>0\<guillemotright> \<and> $1-tr\<acute> =\<^sub>u $tr\<^sub><\<acute> + \<guillemotleft>tt\<^sub>1\<guillemotright>) ;;
+                                      (M\<lbrakk>0,\<guillemotleft>tt\<^sub>p\<guillemotright>,\<guillemotleft>tt\<^sub>0\<guillemotright>,\<guillemotleft>tt\<^sub>1\<guillemotright>/$tr\<^sub><,$tr\<acute>,$0-tr,$1-tr\<rbrakk>)) \<and> $tr\<acute> =\<^sub>u $tr + \<guillemotleft>tt\<^sub>p\<guillemotright>)"
+    by (rel_blast)
+  also have "... = (\<^bold>\<exists> (tt\<^sub>p, tt\<^sub>0, tt\<^sub>1) \<bullet> (((R2(P) \<and> $tr\<acute> =\<^sub>u $tr + \<guillemotleft>tt\<^sub>0\<guillemotright>) \<parallel>\<^sub>s (R2(Q) \<and> $tr\<acute> =\<^sub>u $tr + \<guillemotleft>tt\<^sub>1\<guillemotright>)) ;;
+                                      (M\<lbrakk>0,\<guillemotleft>tt\<^sub>p\<guillemotright>,\<guillemotleft>tt\<^sub>0\<guillemotright>,\<guillemotleft>tt\<^sub>1\<guillemotright>/$tr\<^sub><,$tr\<acute>,$0-tr,$1-tr\<rbrakk>)) \<and> $tr\<acute> =\<^sub>u $tr + \<guillemotleft>tt\<^sub>p\<guillemotright>)"
+    by (rel_auto, blast, metis le_add trace_class.add_diff_cancel_left)
+  also have "... = (\<^bold>\<exists> (tt\<^sub>p, tt\<^sub>0, tt\<^sub>1) \<bullet> ((   ((\<^bold>\<exists> tt\<^sub>0' \<bullet> P\<lbrakk>0,\<guillemotleft>tt\<^sub>0'\<guillemotright>/$tr,$tr\<acute>\<rbrakk> \<and> $tr\<acute> =\<^sub>u $tr + \<guillemotleft>tt\<^sub>0'\<guillemotright>) \<and> $tr\<acute> =\<^sub>u $tr + \<guillemotleft>tt\<^sub>0\<guillemotright>)
+                                       \<parallel>\<^sub>s ((\<^bold>\<exists> tt\<^sub>1' \<bullet> Q\<lbrakk>0,\<guillemotleft>tt\<^sub>1'\<guillemotright>/$tr,$tr\<acute>\<rbrakk> \<and> $tr\<acute> =\<^sub>u $tr + \<guillemotleft>tt\<^sub>1'\<guillemotright>) \<and> $tr\<acute> =\<^sub>u $tr + \<guillemotleft>tt\<^sub>1\<guillemotright>)) ;;
+                                      (M\<lbrakk>0,\<guillemotleft>tt\<^sub>p\<guillemotright>,\<guillemotleft>tt\<^sub>0\<guillemotright>,\<guillemotleft>tt\<^sub>1\<guillemotright>/$tr\<^sub><,$tr\<acute>,$0-tr,$1-tr\<rbrakk>)) \<and> $tr\<acute> =\<^sub>u $tr + \<guillemotleft>tt\<^sub>p\<guillemotright>)"
+    by (simp add: R2_form usubst)
+  also have "... = (\<^bold>\<exists> (tt\<^sub>p, tt\<^sub>0, tt\<^sub>1) \<bullet> ((   (P\<lbrakk>0,\<guillemotleft>tt\<^sub>0\<guillemotright>/$tr,$tr\<acute>\<rbrakk>  \<and> $tr\<acute> =\<^sub>u $tr + \<guillemotleft>tt\<^sub>0\<guillemotright>)
+                                       \<parallel>\<^sub>s (Q\<lbrakk>0,\<guillemotleft>tt\<^sub>1\<guillemotright>/$tr,$tr\<acute>\<rbrakk> \<and> $tr\<acute> =\<^sub>u $tr + \<guillemotleft>tt\<^sub>1\<guillemotright>)) ;;
+                                      (M\<lbrakk>0,\<guillemotleft>tt\<^sub>p\<guillemotright>,\<guillemotleft>tt\<^sub>0\<guillemotright>,\<guillemotleft>tt\<^sub>1\<guillemotright>/$tr\<^sub><,$tr\<acute>,$0-tr,$1-tr\<rbrakk>)) \<and> $tr\<acute> =\<^sub>u $tr + \<guillemotleft>tt\<^sub>p\<guillemotright>)"
+    by (rel_auto, metis left_cancel_monoid_class.add_left_imp_eq, blast)
+  also have "... = R2(P \<parallel>\<^bsub>M\<^esub> Q)"
+    by (rel_auto, blast, metis diff_add_cancel_left')
+  finally show ?thesis ..
+qed
+
+lemma R2m_R2m'_pbm: "(R2(P) \<parallel>\<^bsub>R2m(M)\<^esub> R2(Q)) = (R2(P) \<parallel>\<^bsub>R2m'(M)\<^esub> R2(Q))"
+  by (rel_blast)
+
+lemma R2_par_by_merge [closure]:
+  assumes "P is R2" "Q is R2" "M is R2m"
+  shows "(P \<parallel>\<^bsub>M\<^esub> Q) is R2"
+  by (metis Healthy_def' R2_R2m'_pbm R2m_R2m'_pbm assms(1) assms(2) assms(3))
+
+lemma R2_par_by_merge' [closure]:
+  assumes "P is R2" "Q is R2" "M is R2m'"
+  shows "(P \<parallel>\<^bsub>M\<^esub> Q) is R2"
+  by (metis Healthy_def' R2_R2m'_pbm assms(1) assms(2) assms(3))
+  
+lemma R1m_skip_merge: "R1m(skip\<^sub>m) = skip\<^sub>m"
+  by (rel_auto)
+
+lemma R1m_disj: "R1m(P \<or> Q) = (R1m(P) \<or> R1m(Q))"
+  by (rel_auto)
+
+lemma R1m_conj: "R1m(P \<and> Q) = (R1m(P) \<and> R1m(Q))"
+  by (rel_auto)
+
+lemma R2m_skip_merge: "R2m(skip\<^sub>m) = skip\<^sub>m"
+  apply (rel_auto) using minus_zero_eq by blast
+
+lemma R2m_disj: "R2m(P \<or> Q) = (R2m(P) \<or> R2m(Q))"
+  by (rel_auto)
+
+lemma R2m_conj: "R2m(P \<and> Q) = (R2m(P) \<and> R2m(Q))"
+  by (rel_auto)
+
+definition R3m :: "('t :: trace, '\<alpha>) rp merge \<Rightarrow> ('t, '\<alpha>) rp merge" where
+  [upred_defs]: "R3m(M) = skip\<^sub>m \<triangleleft> $wait\<^sub>< \<triangleright> M"
+
+lemma R3_par_by_merge:
+  assumes
+    "P is R3" "Q is R3" "M is R3m"
+  shows "(P \<parallel>\<^bsub>M\<^esub> Q) is R3"
+proof -
+  have "(P \<parallel>\<^bsub>M\<^esub> Q) = ((P \<parallel>\<^bsub>M\<^esub> Q)\<lbrakk>true/$wait\<rbrakk> \<triangleleft> $wait \<triangleright> (P \<parallel>\<^bsub>M\<^esub> Q))"
+    by (metis cond_L6 cond_var_split in_var_uvar wait_vwb_lens)
+  also have "... = (((R3 P)\<lbrakk>true/$wait\<rbrakk> \<parallel>\<^bsub>(R3m M)\<lbrakk>true/$wait\<^sub><\<rbrakk>\<^esub> (R3 Q)\<lbrakk>true/$wait\<rbrakk>) \<triangleleft> $wait \<triangleright> (P \<parallel>\<^bsub>M\<^esub> Q))"
+    by (subst_tac, simp add: Healthy_if assms)
+  also have "... = ((II\<lbrakk>true/$wait\<rbrakk> \<parallel>\<^bsub>skip\<^sub>m\<lbrakk>true/$wait\<^sub><\<rbrakk>\<^esub> II\<lbrakk>true/$wait\<rbrakk>) \<triangleleft> $wait \<triangleright> (P \<parallel>\<^bsub>M\<^esub> Q))"
+    by (simp add: R3_def R3m_def usubst)
+  also have "... = ((II \<parallel>\<^bsub>skip\<^sub>m\<^esub> II)\<lbrakk>true/$wait\<rbrakk> \<triangleleft> $wait \<triangleright> (P \<parallel>\<^bsub>M\<^esub> Q))"
+    by (subst_tac)
+  also have "... = (II \<triangleleft> $wait \<triangleright> (P \<parallel>\<^bsub>M\<^esub> Q))"
+    by (simp add: cond_var_subst_left par_by_merge_skip)
+  also have "... = R3(P \<parallel>\<^bsub>M\<^esub> Q)"
+    by (simp add: R3_def)
+  finally show ?thesis
+    by (simp add: Healthy_def)
+qed
+
+lemma SymMerge_R1_true [closure]:
+  "M is SymMerge \<Longrightarrow> M ;; R1(true) is SymMerge"
+  by (rel_auto)
+
+end
