theories/reactive/utp_rea_prog.thy
@@ -1,0 +1,385 @@
+section \<open> Reactive Programs \<close>
+
+theory utp_rea_prog
+  imports utp_rea_cond
+begin
+
+subsection \<open> Stateful reactive alphabet \<close>
+
+text \<open> @{term R3} as presented in the UTP book and related publications is not sensitive to state, 
+  although reactive programs often need this property. Thus is is necessary to use a modification 
+  of @{term R3} from Butterfield et al.~\cite{BGW09} that explicitly states that intermediate
+  waiting states do not propogate final state variables. In order to do this we need an additional
+  observational variable that capture the program state that we call $st$. Upon this foundation,
+  we can define operators for reactive programs. \<close>
+
+alphabet 's rsp_vars = "'t rp_vars" +
+  st :: 's
+
+type_synonym ('s,'t,'\<alpha>) rsp = "('t, ('s, '\<alpha>) rsp_vars_scheme) rp"
+type_synonym ('s,'t,'\<alpha>,'\<beta>) rel_rsp  = "(('s,'t,'\<alpha>) rsp, ('s,'t,'\<beta>) rsp) urel"
+type_synonym ('s,'t,'\<alpha>) hrel_rsp  = "('s,'t,'\<alpha>) rsp hrel"
+type_synonym ('s,'t) rdes = "('s,'t,unit) hrel_rsp"
+  
+translations
+  (type) "('s,'t,'\<alpha>) rsp" <= (type) "('t, ('s, '\<alpha>) rsp_vars_ext) rp"
+  (type) "('s,'t,'\<alpha>) rsp" <= (type) "('t, ('s, '\<alpha>) rsp_vars_scheme) rp"
+  (type) "('s,'t,unit) rsp" <= (type) "('t, 's rsp_vars) rp"
+  (type) "('s,'t,'\<alpha>,'\<beta>) rel_rsp" <= (type) "(('s,'t,'\<alpha>) rsp, ('s1,'t1,'\<beta>) rsp) urel"
+  (type) "('s,'t,'\<alpha>) hrel_rsp"  <= (type) "('s, 't, '\<alpha>) rsp hrel"
+  (type) "('s,'t) rdes" <= (type) "('s, 't, unit) hrel_rsp"
+  
+notation rsp_vars_child_lens\<^sub>a ("\<Sigma>\<^sub>s")
+notation rsp_vars_child_lens ("\<Sigma>\<^sub>S")
+
+abbreviation lift_state_rel ("\<lceil>_\<rceil>\<^sub>S")
+where "\<lceil>P\<rceil>\<^sub>S \<equiv> P \<oplus>\<^sub>p (st \<times>\<^sub>L st)"
+
+abbreviation drop_state_rel ("\<lfloor>_\<rfloor>\<^sub>S")
+where "\<lfloor>P\<rfloor>\<^sub>S \<equiv> P \<restriction>\<^sub>e (st \<times>\<^sub>L st)"
+
+abbreviation lift_state_pre ("\<lceil>_\<rceil>\<^sub>S\<^sub><")
+where "\<lceil>p\<rceil>\<^sub>S\<^sub>< \<equiv> \<lceil>\<lceil>p\<rceil>\<^sub><\<rceil>\<^sub>S"
+
+abbreviation drop_state_pre ("\<lfloor>_\<rfloor>\<^sub>S\<^sub><")
+where "\<lfloor>p\<rfloor>\<^sub>S\<^sub>< \<equiv> \<lfloor>\<lfloor>p\<rfloor>\<^sub>S\<rfloor>\<^sub><"
+
+abbreviation lift_state_post ("\<lceil>_\<rceil>\<^sub>S\<^sub>>")
+where "\<lceil>p\<rceil>\<^sub>S\<^sub>> \<equiv> \<lceil>\<lceil>p\<rceil>\<^sub>>\<rceil>\<^sub>S"
+
+abbreviation drop_state_post ("\<lfloor>_\<rfloor>\<^sub>S\<^sub>>")
+where "\<lfloor>p\<rfloor>\<^sub>S\<^sub>> \<equiv> \<lfloor>\<lfloor>p\<rfloor>\<^sub>S\<rfloor>\<^sub>>"
+
+text \<open> Lifting substitutions on the reactive state \<close>
+
+definition usubst_st_lift :: 
+  "'s usubst \<Rightarrow> (('s,'t::trace,'\<alpha>) rsp \<times> ('s,'t,'\<beta>) rsp) usubst"  ("\<lceil>_\<rceil>\<^sub>S\<^sub>\<sigma>") where
+[upred_defs]: "\<lceil>\<sigma>\<rceil>\<^sub>S\<^sub>\<sigma> = \<lceil>\<sigma> \<oplus>\<^sub>s st\<rceil>\<^sub>s"
+
+abbreviation st_subst :: "'s usubst \<Rightarrow> ('s,'t::trace,'\<alpha>) hrel_rsp \<Rightarrow> ('s, 't, '\<alpha>) hrel_rsp" (infixr "\<dagger>\<^sub>S" 80) where
+"\<sigma> \<dagger>\<^sub>S P \<equiv> \<lceil>\<sigma>\<rceil>\<^sub>S\<^sub>\<sigma> \<dagger> P"
+
+translations
+  "\<sigma> \<dagger>\<^sub>S P" <= "\<lceil>\<sigma> \<oplus>\<^sub>s st\<rceil>\<^sub>s \<dagger> P"
+  "\<sigma> \<dagger>\<^sub>S P" <= "\<lceil>\<sigma>\<rceil>\<^sub>S\<^sub>\<sigma> \<dagger> P"
+  
+syntax
+  "_svid_st_alpha"  :: "svid" ("\<Sigma>\<^sub>S")
+
+translations
+  "_svid_st_alpha" => "CONST rsp_vars_child_lens"
+
+interpretation alphabet_state:
+  lens_interp "\<lambda>(ok, wait, tr, r). (ok, wait, tr, st\<^sub>v r, more r)"
+apply (unfold_locales)
+apply (rule injI)
+apply (clarsimp)
+done
+
+interpretation alphabet_state_rel: lens_interp "\<lambda>(ok, ok', wait, wait', tr, tr', r, r').
+  (ok, ok', wait, wait', tr, tr', st\<^sub>v r, st\<^sub>v r', more r, more r')"
+apply (unfold_locales)
+apply (rule injI)
+apply (clarsimp)
+done
+
+lemma st'_unrest_st_lift_pred [unrest]:
+  "$st\<acute> \<sharp> \<lceil>a\<rceil>\<^sub>S\<^sub><"
+  by (pred_auto)
+
+lemma out_alpha_unrest_st_lift_pre [unrest]:
+  "out\<alpha> \<sharp> \<lceil>a\<rceil>\<^sub>S\<^sub><"
+  by (rel_auto)
+    
+lemma st_lift_lemma:
+  "\<lceil>\<sigma>\<rceil>\<^sub>S\<^sub>\<sigma> = \<sigma> \<oplus>\<^sub>s (fst\<^sub>L ;\<^sub>L (st \<times>\<^sub>L st))"
+  by (auto simp add: upred_defs lens_defs prod.case_eq_if)
+    
+lemma unrest_st_lift [unrest]:
+  fixes x :: "'a \<Longrightarrow> ('s, 't::trace, '\<alpha>) rsp \<times> ('s, 't, '\<alpha>) rsp"
+  assumes "x \<bowtie> ($st)\<^sub>v"
+  shows "x \<sharp> \<lceil>\<sigma>\<rceil>\<^sub>S\<^sub>\<sigma>" (is "?P")
+  by (simp add: st_lift_lemma)
+     (metis assms in_var_def in_var_prod_lens lens_comp_left_id st_vwb_lens unrest_subst_alpha_ext vwb_lens_wb)
+  
+lemma st_lift_R1_true_right: "\<lceil>b\<rceil>\<^sub>S\<^sub>< ;; R1(true) = \<lceil>b\<rceil>\<^sub>S\<^sub><"
+  by (rel_auto)
+    
+lemma st_bij_lemma: "bij_lens (st\<^sub>a +\<^sub>L \<Sigma>\<^sub>s)"
+  by (unfold_locales, auto simp add: lens_defs)
+
+lemma rea_lens_equiv_st_rest: "\<Sigma>\<^sub>R \<approx>\<^sub>L st +\<^sub>L \<Sigma>\<^sub>S"
+proof -
+  have "st +\<^sub>L \<Sigma>\<^sub>S = (st\<^sub>a +\<^sub>L \<Sigma>\<^sub>s) ;\<^sub>L \<Sigma>\<^sub>R"
+    by (simp add: plus_lens_distr st_def rsp_vars_child_lens_def)
+  also have "... \<approx>\<^sub>L 1\<^sub>L ;\<^sub>L \<Sigma>\<^sub>R"
+    using lens_equiv_via_bij st_bij_lemma by auto
+  also have "... = \<Sigma>\<^sub>R"
+    by (simp)
+  finally show ?thesis
+    using lens_equiv_sym by blast
+qed
+
+lemma srea_lens_bij: "bij_lens (ok +\<^sub>L wait +\<^sub>L tr +\<^sub>L st +\<^sub>L \<Sigma>\<^sub>S)"
+proof -
+  have "ok +\<^sub>L wait +\<^sub>L tr +\<^sub>L st +\<^sub>L \<Sigma>\<^sub>S \<approx>\<^sub>L ok +\<^sub>L wait +\<^sub>L tr +\<^sub>L \<Sigma>\<^sub>R"
+    by (auto intro!:lens_plus_cong, rule lens_equiv_sym, simp add: rea_lens_equiv_st_rest)
+  also have "... \<approx>\<^sub>L 1\<^sub>L"
+    using bij_lens_equiv_id[of "ok +\<^sub>L wait +\<^sub>L tr +\<^sub>L \<Sigma>\<^sub>R"] by (simp add: rea_lens_bij)
+  finally show ?thesis
+    by (simp add: bij_lens_equiv_id)
+qed
+
+lemma st_qual_alpha [alpha]: "x ;\<^sub>L fst\<^sub>L ;\<^sub>L st \<times>\<^sub>L st = ($st:x)\<^sub>v"
+  by (metis (no_types, hide_lams) in_var_def in_var_prod_lens lens_comp_assoc st_vwb_lens vwb_lens_wb)
+  
+text {* Reactive state assignment *}
+    
+definition rea_assigns :: "('s \<Rightarrow> 's) \<Rightarrow> ('s, 't::trace, '\<alpha>) hrel_rsp" ("\<langle>_\<rangle>\<^sub>r") where
+[upred_defs]: "\<langle>\<sigma>\<rangle>\<^sub>r = ($tr\<acute> =\<^sub>u $tr \<and> \<lceil>\<langle>\<sigma>\<rangle>\<^sub>a\<rceil>\<^sub>S \<and> $\<Sigma>\<^sub>S\<acute> =\<^sub>u $\<Sigma>\<^sub>S)"
+
+syntax
+  "_assign_rea" :: "svids \<Rightarrow> uexprs \<Rightarrow> logic"  ("'(_') :=\<^sub>r '(_')")  
+  "_assign_rea" :: "svids \<Rightarrow> uexprs \<Rightarrow> logic"  (infixr ":=\<^sub>r" 90)
+
+translations
+  "_assign_rea xs vs" => "CONST rea_assigns (_mk_usubst (CONST id) xs vs)"
+  "_assign_rea x v" <= "CONST rea_assigns (CONST subst_upd (CONST id) x v)"
+  "_assign_rea x v" <= "_assign_rea (_spvar x) v"
+  "x,y :=\<^sub>r u,v" <= "CONST rea_assigns (CONST subst_upd (CONST subst_upd (CONST id) (CONST svar x) u) (CONST svar y) v)"
+  
+lemma rea_assigns_RR_closed [closure]: 
+  "\<langle>\<sigma>\<rangle>\<^sub>r is RR"
+  apply (rel_auto) using minus_zero_eq by auto
+    
+lemma id_st_subst [usubst]: 
+  "\<lceil>id\<rceil>\<^sub>S\<^sub>\<sigma> = id"
+  by (pred_auto)
+    
+lemma st_subst_comp [usubst]:
+  "\<lceil>\<sigma>\<rceil>\<^sub>S\<^sub>\<sigma> \<circ> \<lceil>\<rho>\<rceil>\<^sub>S\<^sub>\<sigma> = \<lceil>\<sigma> \<circ> \<rho>\<rceil>\<^sub>S\<^sub>\<sigma>"
+  by (rel_auto)
+    
+lemma st_subst_assigns_rea [usubst]:
+  "\<sigma> \<dagger>\<^sub>S \<langle>\<rho>\<rangle>\<^sub>r = \<langle>\<rho> \<circ> \<sigma>\<rangle>\<^sub>r"
+  by (rel_auto)
+    
+lemma st_subst_rea_skip [usubst]:
+  "\<sigma> \<dagger>\<^sub>S II\<^sub>r = \<langle>\<sigma>\<rangle>\<^sub>r"
+  by (rel_auto)
+    
+lemma rea_assigns_comp [rpred]:
+  assumes "P is RR"
+  shows "\<langle>\<sigma>\<rangle>\<^sub>r ;; P = \<lceil>\<sigma>\<rceil>\<^sub>S\<^sub>\<sigma> \<dagger> P"
+proof -
+  have "\<langle>\<sigma>\<rangle>\<^sub>r ;; (RR P) = \<lceil>\<sigma>\<rceil>\<^sub>S\<^sub>\<sigma> \<dagger> (RR P)"
+    by (rel_auto)
+  thus ?thesis
+    by (metis Healthy_def assms)
+qed
+  
+lemma st_subst_RR [closure]:
+  assumes "P is RR"
+  shows "(\<sigma> \<dagger>\<^sub>S P) is RR"
+proof -
+  have "(\<sigma> \<dagger>\<^sub>S RR(P)) is RR"
+    by (rel_auto)
+  thus ?thesis
+    by (simp add: Healthy_if assms)
+qed
+  
+text {* We guard the reactive conditional condition so that it can't be simplified by alphabet
+  laws unless explicitly simplified. *}
+
+definition lift_cond_srea ("\<lceil>_\<rceil>\<^sub>S\<^sub>\<leftarrow>") where
+[upred_defs]: "\<lceil>b\<rceil>\<^sub>S\<^sub>\<leftarrow> = \<lceil>b\<rceil>\<^sub>S\<^sub><"
+
+lemma unrest_lift_cond_srea [unrest]:
+  "x \<sharp> \<lceil>b\<rceil>\<^sub>S\<^sub>< \<Longrightarrow> x \<sharp> \<lceil>b\<rceil>\<^sub>S\<^sub>\<leftarrow>"
+  by (simp add: lift_cond_srea_def)
+
+lemma subst_lift_cond_srea [usubst]: "\<lceil>\<sigma>\<rceil>\<^sub>S\<^sub>\<sigma> \<dagger> \<lceil>s\<rceil>\<^sub>S\<^sub>\<leftarrow> = \<lceil>\<sigma> \<dagger> s\<rceil>\<^sub>S\<^sub>\<leftarrow>"
+  by (rel_auto)
+    
+abbreviation cond_srea ::
+  "('s,'t::trace,'\<alpha>,'\<beta>) rel_rsp \<Rightarrow>
+  's upred \<Rightarrow>
+  ('s,'t,'\<alpha>,'\<beta>) rel_rsp \<Rightarrow>
+  ('s,'t,'\<alpha>,'\<beta>) rel_rsp" ("(3_ \<triangleleft> _ \<triangleright>\<^sub>R/ _)" [52,0,53] 52) where
+"cond_srea P b Q \<equiv> P \<triangleleft> \<lceil>b\<rceil>\<^sub>S\<^sub>\<leftarrow> \<triangleright> Q"
+
+text {* We introduce state abstraction by creating some lens functors that allow us to lift
+  a lens on the state-space to one on the whole stateful reactive alphabet. *}
+
+definition lmap\<^sub>R :: "('a \<Longrightarrow> 'b) \<Rightarrow> ('t::trace, 'a) rp \<Longrightarrow> ('t, 'b) rp" where
+[lens_defs]: "lmap\<^sub>R = lmap\<^sub>D \<circ> lmap[rp_vars]"
+
+definition map_rsp_st ::
+  "('\<sigma> \<Rightarrow> '\<tau>) \<Rightarrow>
+   ('\<sigma>, '\<alpha>) rsp_vars_scheme \<Rightarrow> ('\<tau>, '\<alpha>) rsp_vars_scheme" where
+[lens_defs]: "map_rsp_st f = (\<lambda>r. \<lparr>st\<^sub>v = f (st\<^sub>v r), \<dots> = rsp_vars.more r\<rparr>)"
+
+definition map_st_lens ::
+  "('\<sigma> \<Longrightarrow> '\<psi>) \<Rightarrow>
+   (('\<sigma>, '\<tau>::trace, '\<alpha>) rsp \<Longrightarrow> ('\<psi>, '\<tau>::trace, '\<alpha>) rsp)" ("map'_st\<^sub>L") where
+[lens_defs]:
+"map_st_lens l = lmap\<^sub>R \<lparr>
+  lens_get = map_rsp_st (get\<^bsub>l\<^esub>),
+  lens_put = map_rsp_st o (put\<^bsub>l\<^esub>) o rsp_vars.st\<^sub>v\<rparr>"
+
+lemma map_set_vwb [simp]: "vwb_lens X \<Longrightarrow> vwb_lens (map_st\<^sub>L X)"
+  apply (unfold_locales, simp_all add: lens_defs des_vars.defs rp_vars.defs rsp_vars.defs)
+  apply (metis des_vars.surjective rp_vars.surjective rsp_vars.surjective)+
+done
+
+abbreviation "abs_st\<^sub>L \<equiv> (map_st\<^sub>L 0\<^sub>L) \<times>\<^sub>L (map_st\<^sub>L 0\<^sub>L)"
+  
+abbreviation abs_st ("\<langle>_\<rangle>\<^sub>S") where
+"abs_st P \<equiv> P \<restriction>\<^sub>e abs_st\<^sub>L"
+  
+text {* Reactive Frames and Extensions *}
+  
+definition rea_frame :: "('a \<Longrightarrow> '\<alpha>) \<Rightarrow> ('\<alpha>, 't::trace) rdes \<Rightarrow> ('\<alpha>, 't) rdes" where
+[upred_defs]: "rea_frame x P = frame (ok +\<^sub>L wait +\<^sub>L tr +\<^sub>L (x ;\<^sub>L st)) P"
+
+definition rea_frame_ext :: "('\<alpha> \<Longrightarrow> '\<beta>) \<Rightarrow> ('\<alpha>, 't::trace) rdes \<Rightarrow> ('\<beta>, 't) rdes" where
+[upred_defs]: "rea_frame_ext a P = rea_frame a (rel_aext P (map_st\<^sub>L a))"
+
+syntax
+  "_rea_frame"     :: "salpha \<Rightarrow> logic \<Rightarrow> logic" ("_:[_]\<^sub>r" [99,0] 100)
+  "_rea_frame_ext" :: "salpha \<Rightarrow> logic \<Rightarrow> logic" ("_:[_]\<^sub>r\<^sup>+" [99,0] 100)
+
+translations
+  "_rea_frame x P" => "CONST rea_frame x P"
+  "_rea_frame (_salphaset (_salphamk x)) P" <= "CONST rea_frame x P"
+  "_rea_frame_ext x P" => "CONST rea_frame_ext x P"
+  "_rea_frame_ext (_salphaset (_salphamk x)) P" <= "CONST rea_frame_ext x P"
+
+lemma rea_frame_RR_closed [closure]: 
+  assumes "P is RR"
+  shows "x:[P]\<^sub>r is RR"
+proof -
+  have "RR(x:[RR P]\<^sub>r) = x:[RR P]\<^sub>r"
+    by (rel_auto)
+  thus ?thesis
+    by (metis Healthy_if Healthy_intro assms)
+qed
+  
+lemma rea_aext_RR [closure]:
+  assumes "P is RR"
+  shows "rel_aext P (map_st\<^sub>L x) is RR"
+proof -
+  have "rel_aext (RR P) (map_st\<^sub>L x) is RR"
+    by (rel_auto)
+  thus ?thesis
+    by (simp add: Healthy_if assms)
+qed
+  
+lemma rea_frame_ext_RR_closed [closure]:
+  "P is RR \<Longrightarrow> x:[P]\<^sub>r\<^sup>+ is RR"
+  by (simp add: rea_frame_ext_def closure)
+  
+lemma rel_aext_st_Instant_closed [closure]:
+  "P is Instant \<Longrightarrow> rel_aext P (map_st\<^sub>L x) is Instant"
+  by (rel_auto)
+
+(*
+lemma rea_frame_commute:
+  assumes "P is RR" "Q is RR" "vwb_lens x" "vwb_lens y"
+          "$st:y \<sharp> P" "$st:x \<sharp> Q" "$st:y\<acute> \<sharp> P" "$st:x\<acute> \<sharp> Q" 
+          "P is Instant" "Q is Instant" "x \<bowtie> y"
+  shows "x:[P]\<^sub>r ;; y:[Q]\<^sub>r = y:[Q]\<^sub>r ;; x:[P]\<^sub>r"     
+proof -
+  have "x:[P]\<^sub>r ;; y:[Q]\<^sub>r = {&tr,&ok,&wait,&st:x}:[P] ;; {&tr,&ok,&wait,&st:y}:[Q]"
+    by (rel_auto)
+  also have "... = {&ok,&wait,&st:x}:[P] ;; {&ok,&wait,&st:y}:[Q]"
+    by (simp add: frame_contract_RID closure assms)
+  also have "... = {&ok,&wait,&st:x}:[RR(P)] ;; {&ok,&wait,&st:y}:[RR(Q)]"
+    by (simp add: assms Healthy_if)
+  also have "... = {&ok,&wait,&st:x}:[RR(P)] ;; {&ok,&wait,&st:y}:[RR(Q)]"
+    by (simp add: assms Healthy_if)    
+  also have "... = {&ok,&wait,&st:y}:[RR(Q)] ;; {&ok,&wait,&st:x}:[RR(P)]"
+    using assms(3-8,11) apply (rel_auto)
+
+  also have "... = {&ok,&wait,&st:y}:[RR(Q)] ;; {&ok,&wait,&st:x}:[RR(P)]"      
+    using assms(3-8,11)
+    apply (rel_auto)
+    
+  also have "... = {&ok,&wait,&st:y}:[Q] ;; {&ok,&wait,&st:x}:[P]"      
+    by (simp add: assms Healthy_if)
+  also have "... = {&tr,&ok,&wait,&st:y}:[Q] ;; {&tr,&ok,&wait,&st:x}:[P]"
+    by (simp add: frame_contract_RID closure assms)
+  also have "... = y:[Q]\<^sub>r ;; x:[P]\<^sub>r"
+    by (rel_auto)
+  finally show ?thesis .
+qed
+  
+lemma rea_frame_ext_commute:
+  assumes "P is RR" "Q is RR" "vwb_lens x" "vwb_lens y"
+          "P is Instant" "Q is Instant" "x \<bowtie> y"
+  shows "x:[P]\<^sub>r\<^sup>+ ;; y:[Q]\<^sub>r\<^sup>+ = y:[Q]\<^sub>r\<^sup>+ ;; x:[P]\<^sub>r\<^sup>+"
+  apply (simp add: rea_frame_ext_def)
+  apply (rule rea_frame_commute)
+  apply (simp_all add: closure assms)
+  apply (rel_auto, simp_all add: assms)
+  apply (rel_auto, simp_all add: assms lens_indep_sym)
+done
+*)    
+  
+lemma rea_frame_ext_false [frame]:
+  "x:[false]\<^sub>r\<^sup>+ = false"
+  by (rel_auto)
+  
+lemma rea_frame_ext_skip [frame]:
+  "vwb_lens x \<Longrightarrow> x:[II\<^sub>r]\<^sub>r\<^sup>+ = II\<^sub>r"
+  by (rel_auto)
+
+lemma rea_frame_ext_assigns [frame]:
+  "vwb_lens x \<Longrightarrow> x:[\<langle>\<sigma>\<rangle>\<^sub>r]\<^sub>r\<^sup>+ = \<langle>\<sigma> \<oplus>\<^sub>s x\<rangle>\<^sub>r"
+  by (rel_auto)
+
+lemma rea_frame_ext_cond [frame]:
+  "x:[P \<triangleleft> b \<triangleright>\<^sub>R Q]\<^sub>r\<^sup>+ = x:[P]\<^sub>r\<^sup>+ \<triangleleft> (b \<oplus>\<^sub>p x) \<triangleright>\<^sub>R x:[Q]\<^sub>r\<^sup>+"
+  by (rel_auto)
+    
+lemma rea_frame_ext_seq [frame]:
+  "vwb_lens x \<Longrightarrow> x:[P ;; Q]\<^sub>r\<^sup>+ = x:[P]\<^sub>r\<^sup>+ ;; x:[Q]\<^sub>r\<^sup>+"
+  apply (simp add: rea_frame_ext_def rea_frame_def alpha frame)
+  apply (subst frame_seq)
+  apply (simp_all add: plus_vwb_lens closure)
+  apply (rel_auto)+
+done
+    
+lemma rea_assigns_st_subst [usubst]:
+  "\<lceil>\<sigma> \<oplus>\<^sub>s st\<rceil>\<^sub>s \<dagger> \<langle>\<rho>\<rangle>\<^sub>r = \<langle>\<rho> \<circ> \<sigma>\<rangle>\<^sub>r"
+  by (rel_auto)
+    
+lemma st_cond_assigns [rpred]:
+  "\<langle>\<sigma>\<rangle>\<^sub>r \<triangleleft> b \<triangleright>\<^sub>R \<langle>\<rho>\<rangle>\<^sub>r = \<langle>\<sigma> \<triangleleft> b \<triangleright>\<^sub>s \<rho>\<rangle>\<^sub>r"
+  by (rel_auto)
+    
+lemma rea_frame_ext_subst_indep [usubst]:
+  assumes "x \<bowtie> y" "\<Sigma> \<sharp> v" "P is RR"
+  shows "\<sigma>(y \<mapsto>\<^sub>s v) \<dagger>\<^sub>S x:[P]\<^sub>r\<^sup>+ = (\<sigma> \<dagger>\<^sub>S x:[P]\<^sub>r\<^sup>+) ;; y :=\<^sub>r v"
+proof -
+  from assms(1-2) have "\<sigma>(y \<mapsto>\<^sub>s v) \<dagger>\<^sub>S x:[RR P]\<^sub>r\<^sup>+ = (\<sigma> \<dagger>\<^sub>S x:[RR P]\<^sub>r\<^sup>+) ;; y :=\<^sub>r v"
+    by (rel_auto, (metis (no_types, lifting) lens_indep.lens_put_comm lens_indep_get)+)
+  thus ?thesis
+    by (simp add: Healthy_if assms)
+qed
+
+lemma rea_frame_ext_subst_within [usubst]:
+  assumes "vwb_lens x" "vwb_lens y" "\<Sigma> \<sharp> v" "P is RR"
+  shows "\<sigma>(x:y \<mapsto>\<^sub>s v) \<dagger>\<^sub>S x:[P]\<^sub>r\<^sup>+ = (\<sigma> \<dagger>\<^sub>S x:[y :=\<^sub>r (v \<restriction>\<^sub>e x) ;; P]\<^sub>r\<^sup>+)"
+proof -
+  from assms(1,3) have "\<sigma>(x:y \<mapsto>\<^sub>s v) \<dagger>\<^sub>S x:[RR P]\<^sub>r\<^sup>+ = (\<sigma> \<dagger>\<^sub>S x:[y :=\<^sub>r (v \<restriction>\<^sub>e x) ;; RR(P)]\<^sub>r\<^sup>+)"
+    by (rel_auto, metis+)
+  thus ?thesis
+    by (simp add: assms Healthy_if)
+qed
+    
+lemma st_subst_lift_cond [usubst]:
+  "\<sigma> \<dagger>\<^sub>S \<lceil>P\<rceil>\<^sub>S\<^sub>\<leftarrow> = \<lceil>\<sigma> \<dagger> P\<rceil>\<^sub>S\<^sub>\<leftarrow>"
+  by (rel_auto)
+
+end
