theories/reactive/utp_rea_rel.thy
@@ -1,0 +1,498 @@
+section \<open> Reactive Relations \<close>
+
+theory utp_rea_rel
+  imports utp_rea_healths
+begin
+
+text \<open> This theory defines a predicate calculus for R1-R2 predicates as an extension of the standard 
+  alphabetised predicate calculus. \<close>
+
+subsection \<open> Healthiness Conditions \<close>
+
+definition RR :: "('t::trace, '\<alpha>, '\<beta>) rel_rp \<Rightarrow> ('t, '\<alpha>, '\<beta>) rel_rp" where
+[upred_defs]: "RR(P) = (\<exists> {$ok,$ok\<acute>,$wait,$wait\<acute>} \<bullet> R2(P))"
+  
+lemma RR_idem: "RR(RR(P)) = RR(P)"
+  by (rel_auto)
+
+lemma RR_Idempotent [closure]: "Idempotent RR"
+  by (simp add: Idempotent_def RR_idem)
+
+lemma RR_Continuous [closure]: "Continuous RR"
+  by (rel_blast)
+    
+lemma R1_RR: "R1(RR(P)) = RR(P)"
+  by (rel_auto)
+    
+lemma R2c_RR: "R2c(RR(P)) = RR(P)"
+  by (rel_auto)
+    
+lemma RR_implies_R1 [closure]: "P is RR \<Longrightarrow> P is R1"
+  by (metis Healthy_def R1_RR)
+  
+lemma RR_implies_R2c: "P is RR \<Longrightarrow> P is R2c"
+  by (metis Healthy_def R2c_RR)
+  
+lemma RR_implies_R2: "P is RR \<Longrightarrow> P is R2"
+  by (metis Healthy_def R1_RR R2_R2c_def R2c_RR)
+
+lemma RR_intro:
+  assumes "$ok \<sharp> P" "$ok\<acute> \<sharp> P" "$wait \<sharp> P" "$wait\<acute> \<sharp> P" "P is R1" "P is R2c"
+  shows "P is RR"
+  by (simp add: RR_def Healthy_def ex_plus R2_R2c_def, simp add: Healthy_if assms ex_unrest)
+    
+lemma RR_R2_intro:
+  assumes "$ok \<sharp> P" "$ok\<acute> \<sharp> P" "$wait \<sharp> P" "$wait\<acute> \<sharp> P" "P is R2"
+  shows "P is RR"
+  by (simp add: RR_def Healthy_def ex_plus, simp add: Healthy_if assms ex_unrest)
+    
+lemma RR_unrests [unrest]: 
+  assumes "P is RR"
+  shows "$ok \<sharp> P" "$ok\<acute> \<sharp> P" "$wait \<sharp> P" "$wait\<acute> \<sharp> P"
+proof -
+  have "$ok \<sharp> RR(P)" "$ok\<acute> \<sharp> RR(P)" "$wait \<sharp> RR(P)" "$wait\<acute> \<sharp> RR(P)"
+    by (simp_all add: RR_def ex_plus unrest)
+  thus "$ok \<sharp> P" "$ok\<acute> \<sharp> P" "$wait \<sharp> P" "$wait\<acute> \<sharp> P"
+    by (simp_all add: assms Healthy_if)
+qed
+
+subsection \<open> Reactive relational operators \<close>
+
+named_theorems rpred
+  
+abbreviation rea_true :: "('t::trace,'\<alpha>,'\<beta>) rel_rp" ("true\<^sub>r") where 
+"true\<^sub>r \<equiv> R1(true)"     
+
+definition rea_not :: "('t::trace,'\<alpha>,'\<beta>) rel_rp \<Rightarrow> ('t,'\<alpha>,'\<beta>) rel_rp" ("\<not>\<^sub>r _" [40] 40) 
+where [upred_defs]: "(\<not>\<^sub>r P) = R1(\<not> P)"
+
+definition rea_diff :: "('t::trace,'\<alpha>,'\<beta>) rel_rp \<Rightarrow> ('t,'\<alpha>,'\<beta>) rel_rp \<Rightarrow> ('t,'\<alpha>,'\<beta>) rel_rp" (infixl "-\<^sub>r" 65)
+where [upred_defs]: "rea_diff P Q = (P \<and> \<not>\<^sub>r Q)"
+  
+definition rea_impl :: 
+  "('t::trace,'\<alpha>,'\<beta>) rel_rp \<Rightarrow> ('t,'\<alpha>,'\<beta>) rel_rp \<Rightarrow> ('t,'\<alpha>,'\<beta>) rel_rp" (infixr "\<Rightarrow>\<^sub>r" 25) 
+where [upred_defs]: "(P \<Rightarrow>\<^sub>r Q) = (\<not>\<^sub>r P \<or> Q)"
+
+definition rea_lift :: "('t::trace,'\<alpha>,'\<beta>) rel_rp \<Rightarrow> ('t,'\<alpha>,'\<beta>) rel_rp" ("[_]\<^sub>r") 
+where [upred_defs]: "[P]\<^sub>r = R1(P)"
+   
+definition rea_skip :: "('t::trace,'\<alpha>) hrel_rp" ("II\<^sub>r") 
+where [upred_defs]: "II\<^sub>r = ($tr\<acute> =\<^sub>u $tr \<and> $\<Sigma>\<^sub>R\<acute> =\<^sub>u $\<Sigma>\<^sub>R)"
+  
+definition rea_assert :: "('t::trace,'\<alpha>) hrel_rp \<Rightarrow> ('t,'\<alpha>) hrel_rp" ("{_}\<^sub>r")
+where [upred_defs]: "{b}\<^sub>r = (II\<^sub>r \<or> \<not>\<^sub>r b)"
+
+definition rea_star :: "_ \<Rightarrow> _"  ("_\<^sup>\<star>\<^sup>r" [999] 999) where
+[upred_defs]: "P\<^sup>\<star>\<^sup>r = P\<^sup>\<star> ;; II\<^sub>r"
+
+text \<open> Trace contribution substitution: make a substitution for the trace contribution lens 
+  @{term tt}, and apply @{term R1} to make the resulting predicate healthy again. \<close>
+  
+definition rea_subst :: "('t::trace, '\<alpha>) hrel_rp \<Rightarrow> ('t, ('t, '\<alpha>) rp) hexpr \<Rightarrow> ('t, '\<alpha>) hrel_rp" ("_\<lbrakk>_\<rbrakk>\<^sub>r" [999,0] 999) 
+where [upred_defs]: "P\<lbrakk>v\<rbrakk>\<^sub>r = R1(P\<lbrakk>v/&tt\<rbrakk>)"
+
+subsection \<open> Unrestriction and substitution laws \<close>
+
+lemma rea_true_unrest [unrest]:
+  "\<lbrakk> x \<bowtie> ($tr)\<^sub>v; x \<bowtie> ($tr\<acute>)\<^sub>v \<rbrakk> \<Longrightarrow> x \<sharp> true\<^sub>r"
+  by (simp add: R1_def unrest lens_indep_sym)
+
+lemma rea_not_unrest [unrest]:
+  "\<lbrakk> x \<bowtie> ($tr)\<^sub>v; x \<bowtie> ($tr\<acute>)\<^sub>v; x \<sharp> P \<rbrakk> \<Longrightarrow> x \<sharp> \<not>\<^sub>r P"
+  by (simp add: rea_not_def R1_def unrest lens_indep_sym)
+
+lemma rea_impl_unrest [unrest]:
+  "\<lbrakk> x \<bowtie> ($tr)\<^sub>v; x \<bowtie> ($tr\<acute>)\<^sub>v; x \<sharp> P; x \<sharp> Q \<rbrakk> \<Longrightarrow> x \<sharp> (P \<Rightarrow>\<^sub>r Q)"
+  by (simp add: rea_impl_def unrest)
+    
+lemma rea_true_usubst [usubst]:
+  "\<lbrakk> $tr \<sharp> \<sigma>; $tr\<acute> \<sharp> \<sigma> \<rbrakk> \<Longrightarrow> \<sigma> \<dagger> true\<^sub>r = true\<^sub>r"
+  by (simp add: R1_def usubst)
+  
+lemma rea_not_usubst [usubst]:
+  "\<lbrakk> $tr \<sharp> \<sigma>; $tr\<acute> \<sharp> \<sigma> \<rbrakk> \<Longrightarrow> \<sigma> \<dagger> (\<not>\<^sub>r P) = (\<not>\<^sub>r \<sigma> \<dagger> P)"
+  by (simp add: rea_not_def R1_def usubst)
+
+lemma rea_impl_usubst [usubst]:
+  "\<lbrakk> $tr \<sharp> \<sigma>; $tr\<acute> \<sharp> \<sigma> \<rbrakk> \<Longrightarrow> \<sigma> \<dagger> (P \<Rightarrow>\<^sub>r Q) = (\<sigma> \<dagger> P \<Rightarrow>\<^sub>r \<sigma> \<dagger> Q)"
+  by (simp add: rea_impl_def usubst R1_def)
+
+lemma rea_true_usubst_tt [usubst]: 
+  "R1(true)\<lbrakk>e/&tt\<rbrakk> = true"
+  by (rel_simp)
+
+lemma unrest_rea_subst [unrest]: 
+  "\<lbrakk> mwb_lens x; x \<bowtie> ($tr)\<^sub>v; x \<bowtie> ($tr\<acute>)\<^sub>v; x \<sharp> v; x \<sharp> P \<rbrakk> \<Longrightarrow>  x \<sharp> P\<lbrakk>v\<rbrakk>\<^sub>r"
+  by (simp add: rea_subst_def R1_def unrest lens_indep_sym)
+
+lemma rea_substs [usubst]: 
+  "true\<^sub>r\<lbrakk>v\<rbrakk>\<^sub>r = true\<^sub>r" "true\<lbrakk>v\<rbrakk>\<^sub>r = true\<^sub>r" "false\<lbrakk>v\<rbrakk>\<^sub>r = false"
+  "(\<not>\<^sub>r P)\<lbrakk>v\<rbrakk>\<^sub>r = (\<not>\<^sub>r P\<lbrakk>v\<rbrakk>\<^sub>r)" "(P \<and> Q)\<lbrakk>v\<rbrakk>\<^sub>r = (P\<lbrakk>v\<rbrakk>\<^sub>r \<and> Q\<lbrakk>v\<rbrakk>\<^sub>r)" "(P \<or> Q)\<lbrakk>v\<rbrakk>\<^sub>r = (P\<lbrakk>v\<rbrakk>\<^sub>r \<or> Q\<lbrakk>v\<rbrakk>\<^sub>r)"
+  "(P \<Rightarrow>\<^sub>r Q)\<lbrakk>v\<rbrakk>\<^sub>r = (P\<lbrakk>v\<rbrakk>\<^sub>r \<Rightarrow>\<^sub>r Q\<lbrakk>v\<rbrakk>\<^sub>r)"
+  by rel_auto+
+
+lemma rea_substs_lattice [usubst]:
+  "(\<Sqinter> i \<bullet> P(i))\<lbrakk>v\<rbrakk>\<^sub>r   = (\<Sqinter> i \<bullet> (P(i))\<lbrakk>v\<rbrakk>\<^sub>r)"
+  "(\<Sqinter> i\<in>A \<bullet> P(i))\<lbrakk>v\<rbrakk>\<^sub>r = (\<Sqinter> i\<in>A \<bullet> (P(i))\<lbrakk>v\<rbrakk>\<^sub>r)"
+  "(\<Squnion> i \<bullet> P(i))\<lbrakk>v\<rbrakk>\<^sub>r   = (\<Squnion> i \<bullet> (P(i))\<lbrakk>v\<rbrakk>\<^sub>r)"
+   by (rel_auto)+
+    
+lemma rea_subst_USUP_set [usubst]:
+  "A \<noteq> {} \<Longrightarrow> (\<Squnion> i\<in>A \<bullet> P(i))\<lbrakk>v\<rbrakk>\<^sub>r   = (\<Squnion> i\<in>A \<bullet> (P(i))\<lbrakk>v\<rbrakk>\<^sub>r)"
+  by (rel_auto)+
+
+subsection \<open> Closure laws \<close>
+
+lemma rea_lift_R1 [closure]: "[P]\<^sub>r is R1"
+  by (rel_simp)
+    
+lemma R1_rea_not: "R1(\<not>\<^sub>r P) = (\<not>\<^sub>r P)"
+  by rel_auto
+    
+lemma R1_rea_not': "R1(\<not>\<^sub>r P) = (\<not>\<^sub>r R1(P))"
+  by rel_auto  
+  
+lemma R2c_rea_not: "R2c(\<not>\<^sub>r P) = (\<not>\<^sub>r R2c(P))"
+  by rel_auto
+
+lemma RR_rea_not: "RR(\<not>\<^sub>r RR(P)) = (\<not>\<^sub>r RR(P))"
+  by (rel_auto)
+    
+lemma R1_rea_impl: "R1(P \<Rightarrow>\<^sub>r Q) = (P \<Rightarrow>\<^sub>r R1(Q))"
+  by (rel_auto)
+
+lemma R1_rea_impl': "R1(P \<Rightarrow>\<^sub>r Q) = (R1(P) \<Rightarrow>\<^sub>r R1(Q))"
+  by (rel_auto)
+    
+lemma R2c_rea_impl: "R2c(P \<Rightarrow>\<^sub>r Q) = (R2c(P) \<Rightarrow>\<^sub>r R2c(Q))"
+  by (rel_auto)
+
+lemma RR_rea_impl: "RR(RR(P) \<Rightarrow>\<^sub>r RR(Q)) = (RR(P) \<Rightarrow>\<^sub>r RR(Q))"
+  by (rel_auto)
+ 
+lemma rea_true_R1 [closure]: "true\<^sub>r is R1"
+  by (rel_auto)
+  
+lemma rea_true_R2c [closure]: "true\<^sub>r is R2c"
+  by (rel_auto)
+    
+lemma rea_true_RR [closure]: "true\<^sub>r is RR"
+  by (rel_auto)
+     
+lemma rea_not_R1 [closure]: "\<not>\<^sub>r P is R1"
+  by (rel_auto)
+
+lemma rea_not_R2c [closure]: "P is R2c \<Longrightarrow> \<not>\<^sub>r P is R2c"
+  by (simp add: Healthy_def rea_not_def R1_R2c_commute[THEN sym] R2c_not)
+   
+lemma rea_not_R2_closed [closure]:
+  "P is R2 \<Longrightarrow> (\<not>\<^sub>r P) is R2"
+  by (simp add: Healthy_def' R1_rea_not' R2_R2c_def R2c_rea_not)
+
+lemma rea_no_RR [closure]:
+  "\<lbrakk> P is RR \<rbrakk> \<Longrightarrow> (\<not>\<^sub>r P) is RR"
+  by (metis Healthy_def' RR_rea_not)
+
+lemma rea_impl_R1 [closure]: 
+  "Q is R1 \<Longrightarrow> (P \<Rightarrow>\<^sub>r Q) is R1"
+  by (rel_blast)
+
+lemma rea_impl_R2c [closure]: 
+  "\<lbrakk> P is R2c; Q is R2c \<rbrakk> \<Longrightarrow> (P \<Rightarrow>\<^sub>r Q) is R2c"
+  by (simp add: rea_impl_def Healthy_def rea_not_def R1_R2c_commute[THEN sym] R2c_not R2c_disj)
+
+lemma rea_impl_R2 [closure]: 
+  "\<lbrakk> P is R2; Q is R2 \<rbrakk> \<Longrightarrow> (P \<Rightarrow>\<^sub>r Q) is R2"
+  by (rel_blast)
+
+lemma rea_impl_RR [closure]:
+  "\<lbrakk> P is RR; Q is RR \<rbrakk> \<Longrightarrow> (P \<Rightarrow>\<^sub>r Q) is RR"
+  by (metis Healthy_def' RR_rea_impl)
+  
+lemma conj_RR [closure]:
+  "\<lbrakk> P is RR; Q is RR \<rbrakk> \<Longrightarrow> (P \<and> Q) is RR"
+  by (meson RR_implies_R1 RR_implies_R2c RR_intro RR_unrests(1-4) conj_R1_closed_1 conj_R2c_closed unrest_conj)
+
+lemma disj_RR [closure]:
+  "\<lbrakk> P is RR; Q is RR \<rbrakk> \<Longrightarrow> (P \<or> Q) is RR"
+  by (metis Healthy_def' R1_RR R1_idem R1_rea_not' RR_rea_impl RR_rea_not disj_comm double_negation rea_impl_def rea_not_def)
+
+lemma USUP_mem_RR_closed [closure]:
+  assumes "\<And> i. P i is RR" "A \<noteq> {}"
+  shows "(\<Squnion> i\<in>A \<bullet> P(i)) is RR"
+proof -
+  have 1:"(\<Squnion> i\<in>A \<bullet> P(i)) is R1"
+    by (unfold Healthy_def, subst R1_UINF, simp_all add: Healthy_if assms closure)
+  have 2:"(\<Squnion> i\<in>A \<bullet> P(i)) is R2c"
+    by (unfold Healthy_def, subst R2c_UINF, simp_all add: Healthy_if assms RR_implies_R2c closure)
+  show ?thesis
+    using 1 2 by (rule_tac RR_intro, simp_all add: unrest assms)
+qed
+
+lemma USUP_ind_RR_closed [closure]:
+  assumes "\<And> i. P i is RR"
+  shows "(\<Squnion> i \<bullet> P(i)) is RR"
+  using USUP_mem_RR_closed[of P UNIV] by (simp add: assms)
+
+lemma UINF_mem_RR_closed [closure]:
+  assumes "\<And> i. P i is RR"
+  shows "(\<Sqinter> i\<in>A \<bullet> P(i)) is RR"
+proof -
+  have 1:"(\<Sqinter> i\<in>A \<bullet> P(i)) is R1"
+    by (unfold Healthy_def, subst R1_USUP, simp_all add: Healthy_if assms closure)
+  have 2:"(\<Sqinter> i\<in>A \<bullet> P(i)) is R2c"
+    by (unfold Healthy_def, subst R2c_USUP, simp_all add: Healthy_if assms RR_implies_R2c closure)
+  show ?thesis
+    using 1 2 by (rule_tac RR_intro, simp_all add: unrest assms)
+qed
+    
+lemma UINF_ind_RR_closed [closure]:
+  assumes "\<And> i. P i is RR"
+  shows "(\<Sqinter> i \<bullet> P(i)) is RR"
+  using UINF_mem_RR_closed[of P UNIV] by (simp add: assms)
+    
+lemma USUP_elem_RR [closure]: 
+  assumes "\<And> i. P i is RR" "A \<noteq> {}"
+  shows "(\<Squnion> i \<in> A \<bullet> P i) is RR"
+proof -
+  have 1:"(\<Squnion> i\<in>A \<bullet> P(i)) is R1"
+    by (unfold Healthy_def, subst R1_UINF, simp_all add: Healthy_if assms closure)
+  have 2:"(\<Squnion> i\<in>A \<bullet> P(i)) is R2c"
+    by (unfold Healthy_def, subst R2c_UINF, simp_all add: Healthy_if assms RR_implies_R2c closure)
+  show ?thesis
+    using 1 2 by (rule_tac RR_intro, simp_all add: unrest assms)
+qed
+
+lemma seq_RR_closed [closure]: 
+  assumes "P is RR" "Q is RR"
+  shows "P ;; Q is RR"
+  unfolding Healthy_def
+  by (simp add: RR_def  Healthy_if assms closure RR_implies_R2 ex_unrest unrest)
+    
+lemma power_Suc_RR_closed [closure]:
+  "P is RR \<Longrightarrow> P ;; P \<^bold>^ i is RR"
+  by (induct i, simp_all add: closure)
+    
+lemma seqr_iter_RR_closed [closure]:
+  "\<lbrakk> I \<noteq> []; \<And> i. i \<in> set(I) \<Longrightarrow> P(i) is RR \<rbrakk> \<Longrightarrow> (;; i : I \<bullet> P(i)) is RR"
+  apply (induct I, simp_all)
+  apply (rename_tac i I)
+  apply (case_tac I)
+  apply (simp_all add: seq_RR_closed)
+done
+    
+lemma cond_tt_RR_closed [closure]: 
+  assumes "P is RR" "Q is RR"
+  shows "P \<triangleleft> $tr\<acute> =\<^sub>u $tr \<triangleright> Q is RR"
+  apply (rule RR_intro)
+  apply (simp_all add: unrest assms)
+  apply (simp_all add: Healthy_def) 
+  apply (simp_all add: R1_cond R2c_condr Healthy_if assms RR_implies_R2c closure R2c_tr'_minus_tr)
+done
+
+lemma rea_skip_RR [closure]:
+  "II\<^sub>r is RR"
+  apply (rel_auto) using minus_zero_eq by blast
+
+lemma tr'_eq_tr_RR_closed [closure]: "$tr\<acute> =\<^sub>u $tr is RR"
+  apply (rel_auto) using minus_zero_eq by auto
+
+lemma inf_RR_closed [closure]: 
+  "\<lbrakk> P is RR; Q is RR \<rbrakk> \<Longrightarrow> P \<sqinter> Q is RR"
+  by (simp add: disj_RR uinf_or)
+  
+lemma rea_assert_RR_closed [closure]:
+  assumes "b is RR"
+  shows "{b}\<^sub>r is RR"
+  by (simp add: closure assms rea_assert_def)
+  
+lemma upower_RR_closed [closure]:
+  "\<lbrakk> i > 0; P is RR \<rbrakk> \<Longrightarrow> P \<^bold>^ i is RR"
+  apply (induct i, simp_all)
+  apply (rename_tac i)
+  apply (case_tac "i = 0")
+   apply (simp_all add: closure)
+done
+  
+lemma ustar_right_RR_closed [closure]:
+  assumes "P is RR" "Q is RR"
+  shows "P ;; Q\<^sup>\<star> is RR"
+proof -
+  have "P ;; Q\<^sup>\<star> = P ;; (\<Sqinter> i \<in> {0..} \<bullet> Q \<^bold>^ i)"
+    by (simp add: ustar_def)
+  also have "... = P ;; (II \<sqinter> (\<Sqinter> i \<in> {1..} \<bullet> Q \<^bold>^ i))"
+    by (metis One_nat_def UINF_atLeast_first upred_semiring.power_0)
+  also have "... = (P \<or> P ;; (\<Sqinter> i \<in> {1..} \<bullet> Q \<^bold>^ i))"
+    by (simp add: disj_upred_def[THEN sym] seqr_or_distr)
+  also have "... is RR"
+  proof -
+    have "(\<Sqinter> i \<in> {1..} \<bullet> Q \<^bold>^ i) is RR"
+      by (rule UINF_mem_Continuous_closed, simp_all add: assms closure)
+    thus ?thesis
+      by (simp add: assms closure)
+  qed
+  finally show ?thesis .
+qed
+
+lemma ustar_left_RR_closed [closure]:
+  assumes "P is RR" "Q is RR"
+  shows "P\<^sup>\<star> ;; Q is RR"
+proof -
+  have "P\<^sup>\<star> ;; Q = (\<Sqinter> i \<in> {0..} \<bullet> P \<^bold>^ i) ;; Q"
+    by (simp add: ustar_def)
+  also have "... = (II \<sqinter> (\<Sqinter> i \<in> {1..} \<bullet> P \<^bold>^ i)) ;; Q"
+    by (metis One_nat_def UINF_atLeast_first upred_semiring.power_0)
+  also have "... = (Q \<or> (\<Sqinter> i \<in> {1..} \<bullet> P \<^bold>^ i) ;; Q)"
+    by (simp add: disj_upred_def[THEN sym] seqr_or_distl)
+  also have "... is RR"
+  proof -
+    have "(\<Sqinter> i \<in> {1..} \<bullet> P \<^bold>^ i) is RR"
+      by (rule UINF_mem_Continuous_closed, simp_all add: assms closure)
+    thus ?thesis
+      by (simp add: assms closure)
+  qed
+  finally show ?thesis .
+qed
+
+lemma rea_star_RR_closed [closure]: 
+  "P is RR \<Longrightarrow> P\<^sup>\<star>\<^sup>r is RR"
+  by (simp add: rea_skip_RR rea_star_def ustar_left_RR_closed)
+
+lemma uplus_RR_closed [closure]: "P is RR \<Longrightarrow> P\<^sup>+ is RR"
+  by (simp add: uplus_def ustar_right_RR_closed)
+
+lemma trace_ext_prefix_RR [closure]: 
+  "\<lbrakk> $tr \<sharp> e; $ok \<sharp> e; $wait \<sharp> e; out\<alpha> \<sharp> e \<rbrakk> \<Longrightarrow> $tr ^\<^sub>u e \<le>\<^sub>u $tr\<acute> is RR"
+  apply (rel_auto)
+  apply (metis (no_types, lifting) Prefix_Order.same_prefix_prefix less_eq_list_def prefix_concat_minus zero_list_def)
+  apply (metis append_minus list_append_prefixD minus_cancel_le order_refl)
+done  
+
+lemma rea_subst_R1_closed [closure]: "P\<lbrakk>v\<rbrakk>\<^sub>r is R1"
+  by (rel_auto)
+
+subsection \<open> Reactive relational calculus \<close>
+
+lemma rea_skip_unit [rpred]:
+  assumes "P is RR"
+  shows "P ;; II\<^sub>r = P" "II\<^sub>r ;; P = P"
+proof -
+  have 1: "RR(P) ;; II\<^sub>r = RR(P)"
+    by (rel_auto)
+  have 2: "II\<^sub>r ;; RR(P) = RR(P)"
+    by (rel_auto)
+  from 1 2 show "P ;; II\<^sub>r = P" "II\<^sub>r ;; P = P"
+    by (simp_all add: Healthy_if assms)
+qed
+  
+lemma rea_star_unfoldl:
+  "P is RR \<Longrightarrow> P\<^sup>\<star>\<^sup>r = II\<^sub>r \<sqinter> (P ;; P\<^sup>\<star>\<^sup>r)"
+  by (metis (no_types, lifting) rea_star_def seqr_assoc seqr_left_unit upred_semiring.distrib_right ustar_unfoldl)
+ 
+lemma rea_uplus_unfold: "P is RR \<Longrightarrow> P\<^sup>+ = P ;; P\<^sup>\<star>\<^sup>r"
+  by (simp add: RA1 rea_skip_unit(1) rea_star_def uplus_def ustar_right_RR_closed)
+    
+lemma rea_true_conj [rpred]: 
+  assumes "P is R1"
+  shows "(true\<^sub>r \<and> P) = P" "(P \<and> true\<^sub>r) = P"
+  using assms
+  by (simp_all add: Healthy_def R1_def utp_pred_laws.inf_commute) 
+
+lemma rea_true_disj [rpred]: 
+  assumes "P is R1"
+  shows "(true\<^sub>r \<or> P) = true\<^sub>r" "(P \<or> true\<^sub>r) = true\<^sub>r"
+  using assms by (metis Healthy_def R1_disj disj_comm true_disj_zero)+
+  
+lemma rea_not_not [rpred]: "P is R1 \<Longrightarrow> (\<not>\<^sub>r \<not>\<^sub>r P) = P"
+  by (simp add: rea_not_def R1_negate_R1 Healthy_if)
+    
+lemma rea_not_rea_true [simp]: "(\<not>\<^sub>r true\<^sub>r) = false"
+  by (simp add: rea_not_def R1_negate_R1 R1_false)
+    
+lemma rea_not_false [simp]: "(\<not>\<^sub>r false) = true\<^sub>r"
+  by (simp add: rea_not_def)
+    
+lemma rea_true_impl [rpred]:
+  "P is R1 \<Longrightarrow> (true\<^sub>r \<Rightarrow>\<^sub>r P) = P"
+  by (simp add: rea_not_def rea_impl_def R1_negate_R1 R1_false Healthy_if)
+
+lemma rea_true_impl' [rpred]:
+  "P is R1 \<Longrightarrow>(true \<Rightarrow>\<^sub>r P) = P"
+  by (simp add: rea_not_def rea_impl_def R1_negate_R1 R1_false Healthy_if)
+    
+lemma rea_false_impl [rpred]:
+  "P is R1 \<Longrightarrow> (false \<Rightarrow>\<^sub>r P) = true\<^sub>r"
+  by (simp add: rea_impl_def rpred Healthy_if)
+   
+lemma rea_impl_true [simp]: "(P \<Rightarrow>\<^sub>r true\<^sub>r) = true\<^sub>r"
+  by (rel_auto)
+    
+lemma rea_impl_false [simp]: "(P \<Rightarrow>\<^sub>r false) = (\<not>\<^sub>r P)"
+  by (rel_simp)
+    
+lemma rea_imp_refl [rpred]: "P is R1 \<Longrightarrow> (P \<Rightarrow>\<^sub>r P) = true\<^sub>r"
+  by (rel_blast)
+    
+lemma rea_not_true [simp]: "(\<not>\<^sub>r true) = false"
+  by (rel_auto)
+    
+lemma rea_not_demorgan1 [simp]:
+  "(\<not>\<^sub>r (P \<and> Q)) = (\<not>\<^sub>r P \<or> \<not>\<^sub>r Q)"
+  by (rel_auto)
+
+lemma rea_not_demorgan2 [simp]:
+  "(\<not>\<^sub>r (P \<or> Q)) = (\<not>\<^sub>r P \<and> \<not>\<^sub>r Q)"
+  by (rel_auto)
+
+lemma rea_not_or [rpred]:
+  "P is R1 \<Longrightarrow> (P \<or> \<not>\<^sub>r P) = true\<^sub>r"
+  by (rel_blast)
+
+lemma rea_not_and [simp]:
+  "(P \<and> \<not>\<^sub>r P) = false"
+  by (rel_auto)
+    
+lemma rea_not_INFIMUM [simp]:
+  "(\<not>\<^sub>r (\<Squnion>i\<in>A. Q(i))) = (\<Sqinter>i\<in>A. \<not>\<^sub>r Q(i))"
+  by (rel_auto)
+
+lemma rea_not_USUP [simp]:
+  "(\<not>\<^sub>r (\<Squnion>i\<in>A \<bullet> Q(i))) = (\<Sqinter>i\<in>A \<bullet> \<not>\<^sub>r Q(i))"
+  by (rel_auto)
+    
+lemma rea_not_SUPREMUM [simp]:
+  "A \<noteq> {} \<Longrightarrow> (\<not>\<^sub>r (\<Sqinter>i\<in>A. Q(i))) = (\<Squnion>i\<in>A. \<not>\<^sub>r Q(i))"
+  by (rel_auto)
+
+lemma rea_not_UINF [simp]:
+  "A \<noteq> {} \<Longrightarrow> (\<not>\<^sub>r (\<Sqinter>i\<in>A \<bullet> Q(i))) = (\<Squnion>i\<in>A \<bullet> \<not>\<^sub>r Q(i))"
+  by (rel_auto)
+
+lemma USUP_mem_rea_true [simp]: "A \<noteq> {} \<Longrightarrow> (\<Squnion> i \<in> A \<bullet> true\<^sub>r) = true\<^sub>r"
+  by (rel_auto)
+
+lemma USUP_ind_rea_true [simp]: "(\<Squnion> i \<bullet> true\<^sub>r) = true\<^sub>r"
+  by (rel_auto)
+    
+lemma UINF_ind_rea_true [rpred]: "A \<noteq> {} \<Longrightarrow> (\<Sqinter> i\<in>A \<bullet> true\<^sub>r) = true\<^sub>r"
+  by (rel_auto)
+    
+lemma rea_assert_true:
+  "{true\<^sub>r}\<^sub>r = II\<^sub>r"
+  by (rel_auto)
+
+lemma rea_false_true:
+  "{false}\<^sub>r = true\<^sub>r"
+  by (rel_auto)
+    
+subsection \<open> Instantaneous Reactive Relations \<close>
+
+text \<open> Instantaneous Reactive Relations, where the trace stays the same. \<close>
+  
+abbreviation Instant :: "('t::trace, '\<alpha>) hrel_rp \<Rightarrow> ('t, '\<alpha>) hrel_rp" where
+"Instant(P) \<equiv> RID(tr)(P)"
+
+lemma skip_rea_Instant [closure]: "II\<^sub>r is Instant"
+  by (rel_auto)
+
+end
