theories/reactive/utp_rea_wp.thy
@@ -1,0 +1,123 @@
+theory utp_rea_wp
+  imports utp_rea_prog
+begin
+
+definition wp_rea ::
+  "('t::trace, '\<alpha>) hrel_rp \<Rightarrow>  
+   ('t, '\<alpha>) hrel_rp \<Rightarrow> 
+   ('t, '\<alpha>) hrel_rp" (infix "wp\<^sub>r" 60)
+where [upred_defs]: "P wp\<^sub>r Q = (\<not>\<^sub>r P ;; (\<not>\<^sub>r Q))"
+
+lemma in_var_unrest_wp_rea [unrest]: "\<lbrakk> $x \<sharp> P; tr \<bowtie> x \<rbrakk> \<Longrightarrow> $x \<sharp> (P wp\<^sub>r Q)"
+  by (simp add: wp_rea_def unrest R1_def rea_not_def)
+
+lemma out_var_unrest_wp_rea [unrest]: "\<lbrakk> $x\<acute> \<sharp> Q; tr \<bowtie> x \<rbrakk> \<Longrightarrow> $x\<acute> \<sharp> (P wp\<^sub>r Q)"
+  by (simp add: wp_rea_def unrest R1_def rea_not_def)
+  
+lemma wp_rea_R1 [closure]: "P wp\<^sub>r Q is R1"
+  by (rel_auto)
+
+lemma wp_rea_RR_closed [closure]: "\<lbrakk> P is RR; Q is RR \<rbrakk> \<Longrightarrow> P wp\<^sub>r Q is RR"
+  by (simp add: wp_rea_def closure)    
+
+lemma wpR_R1_right [wp]:
+  "P wp\<^sub>r R1(Q) = P wp\<^sub>r Q"
+  by (rel_auto)
+
+lemma wp_rea_true [wp]: "P wp\<^sub>r true = true\<^sub>r"
+  by (rel_auto)
+    
+lemma wp_rea_conj [wp]: "P wp\<^sub>r (Q \<and> R) = (P wp\<^sub>r Q \<and> P wp\<^sub>r R)"
+  by (simp add: wp_rea_def seqr_or_distr)
+    
+lemma wp_rea_USUP_mem [wp]: 
+  "A \<noteq> {} \<Longrightarrow> P wp\<^sub>r (\<Squnion> i\<in>A \<bullet> Q(i)) = (\<Squnion> i\<in>A \<bullet> P wp\<^sub>r Q(i))"
+  by (simp add: wp_rea_def seq_UINF_distl)
+    
+lemma wp_rea_div [wp]:
+  "(\<not>\<^sub>r P ;; true\<^sub>r) = true\<^sub>r \<Longrightarrow> true\<^sub>r wp\<^sub>r P = false"
+  by (simp add: wp_rea_def rpred, rel_blast)
+
+lemma wp_rea_cond [wp]:
+  "out\<alpha> \<sharp> b \<Longrightarrow> (P \<triangleleft> b \<triangleright> Q) wp\<^sub>r R = P wp\<^sub>r R \<triangleleft> b \<triangleright> Q wp\<^sub>r R"
+  by (simp add: wp_rea_def cond_seq_left_distr, rel_auto)
+    
+lemma wp_rea_RC_false [wp]: 
+  "P is RC \<Longrightarrow> (\<not>\<^sub>r P) wp\<^sub>r false = P"
+  by (metis Healthy_if RC1_def RC_implies_RC1 rea_not_false wp_rea_def)
+    
+lemma wp_rea_seq [wp]:
+  assumes "Q is R1"
+  shows "(P ;; Q) wp\<^sub>r R = P wp\<^sub>r (Q wp\<^sub>r R)" (is "?lhs = ?rhs")
+proof -
+  have "?rhs = R1 (\<not> P ;; R1 (Q ;; R1 (\<not> R)))"
+    by (simp add: wp_rea_def rea_not_def R1_negate_R1 assms)
+  also have "... = R1 (\<not> P ;; (Q ;; R1 (\<not> R)))"
+    by (metis Healthy_if R1_seqr assms)
+  also have "... = R1 (\<not> (P ;; Q) ;; R1 (\<not> R))"
+    by (simp add: seqr_assoc)
+  finally show ?thesis
+    by (simp add: wp_rea_def rea_not_def)
+qed
+  
+lemma wp_rea_skip [wp]:
+  assumes "Q is R1"
+  shows "II wp\<^sub>r Q = Q"
+  by (simp add: wp_rea_def rpred assms Healthy_if)
+
+lemma wp_rea_rea_skip [wp]:
+  assumes "Q is RR"
+  shows "II\<^sub>r wp\<^sub>r Q = Q"
+  by (simp add: wp_rea_def rpred closure assms Healthy_if)
+    
+lemma power_wp_rea_RR_closed [closure]: 
+  "\<lbrakk> R is RR; P is RR \<rbrakk> \<Longrightarrow> R \<^bold>^ i wp\<^sub>r P is RR"
+  by (induct i, simp_all add: wp closure)
+    
+lemma wp_rea_rea_assigns [wp]:
+  assumes "P is RR"
+  shows "\<langle>\<sigma>\<rangle>\<^sub>r wp\<^sub>r P = \<lceil>\<sigma>\<rceil>\<^sub>S\<^sub>\<sigma> \<dagger> P"
+proof -
+  have "\<langle>\<sigma>\<rangle>\<^sub>r wp\<^sub>r (RR P) = \<lceil>\<sigma>\<rceil>\<^sub>S\<^sub>\<sigma> \<dagger> (RR P)"
+    by (rel_auto)
+  thus ?thesis
+    by (metis Healthy_def assms)
+qed
+  
+lemma wp_rea_miracle [wp]: "false wp\<^sub>r Q = true\<^sub>r"
+  by (simp add: wp_rea_def)
+
+lemma wp_rea_choice [wp]: "(P \<or> Q) wp\<^sub>r R = (P wp\<^sub>r R \<and> Q wp\<^sub>r R)"
+  by (rel_blast)
+
+lemma wp_rea_UINF [wp]:
+  assumes "A \<noteq> {}"
+  shows "(\<Sqinter> x\<in>A \<bullet> P(x)) wp\<^sub>r Q = (\<Squnion> x\<in>A \<bullet> P(x) wp\<^sub>r Q)"
+  by (simp add: wp_rea_def rea_not_def seq_UINF_distr not_UINF R1_UINF assms)
+
+lemma wp_rea_R2_closed [closure]:
+  "\<lbrakk> P is R2; Q is R2 \<rbrakk> \<Longrightarrow> P wp\<^sub>r Q is R2"
+  by (simp add: wp_rea_def closure)
+
+lemma wp_rea_false_RC1': "P is R2 \<Longrightarrow> RC1(P wp\<^sub>r false) = P wp\<^sub>r false"
+  by (simp add: wp_rea_def RC1_def closure rpred seqr_assoc)
+    
+lemma wp_rea_false_RC1: "P is R2 \<Longrightarrow> P wp\<^sub>r false is RC1"
+  by (simp add :Healthy_def wp_rea_false_RC1')
+  
+lemma wp_rea_false_RR:
+  "\<lbrakk> $ok \<sharp> P; $wait \<sharp> P; P is R2 \<rbrakk> \<Longrightarrow> P wp\<^sub>r false is RR"
+  by (rule RR_R2_intro, simp_all add: unrest closure)
+
+lemma wp_rea_false_RC:
+  "\<lbrakk> $ok \<sharp> P; $wait \<sharp> P; P is R2 \<rbrakk> \<Longrightarrow> P wp\<^sub>r false is RC"
+  by (rule RC_intro', simp_all add:  wp_rea_false_RC1 wp_rea_false_RR)
+ 
+lemma wp_rea_RC1: "\<lbrakk> P is RR; Q is RC \<rbrakk> \<Longrightarrow> P wp\<^sub>r Q is RC1"
+  by (rule Healthy_intro, simp add: wp_rea_def RC1_def rpred closure seqr_assoc RC1_prop RC_implies_RC1)
+    
+lemma wp_rea_RC [closure]: "\<lbrakk> P is RR; Q is RC \<rbrakk> \<Longrightarrow> P wp\<^sub>r Q is RC"
+  by (rule RC_intro', simp_all add: wp_rea_RC1 closure)
+
+
+end
