theories/utp_csp.thy
@@ -419,29 +419,29 @@ proof -
     by (simp add: Healthy_if assms)
 qed
     
-lemma wpR_csp_do_lemma:
+lemma wp_rea_csp_do_lemma:
   fixes P :: "('\<sigma>, '\<phi>) action"
   assumes "$ok \<sharp> P" "$wait \<sharp> P" "$ref \<sharp> P"
   shows "(\<lceil>\<langle>\<sigma>\<rangle>\<^sub>a\<rceil>\<^sub>S \<and> $tr\<acute> =\<^sub>u $tr ^\<^sub>u \<lceil>t\<rceil>\<^sub>S\<^sub><) ;; P = (\<lceil>\<sigma>\<rceil>\<^sub>S\<^sub>\<sigma> \<dagger> P)\<lbrakk>$tr ^\<^sub>u \<lceil>t\<rceil>\<^sub>S\<^sub></$tr\<rbrakk>"
   using assms by (rel_auto, meson)
     
-lemma wpR_csp_do [wp]:
+lemma wp_rea_csp_do [wp]:
   fixes P :: "('\<sigma>, '\<phi>) action"
   assumes "P is CRR"
-  shows "\<Phi>(s,\<sigma>,t) wp\<^sub>R P = (\<I>(s,t) \<Rightarrow>\<^sub>r (\<lceil>\<sigma>\<rceil>\<^sub>S\<^sub>\<sigma> \<dagger> P)\<lbrakk>t\<rbrakk>\<^sub>t)"
+  shows "\<Phi>(s,\<sigma>,t) wp\<^sub>r P = (\<I>(s,t) \<Rightarrow>\<^sub>r (\<lceil>\<sigma>\<rceil>\<^sub>S\<^sub>\<sigma> \<dagger> P)\<lbrakk>t\<rbrakk>\<^sub>t)"
 proof -
-  have "\<Phi>(s,\<sigma>,t) wp\<^sub>R CRR(P) = (\<I>(s,t) \<Rightarrow>\<^sub>r (\<lceil>\<sigma>\<rceil>\<^sub>S\<^sub>\<sigma> \<dagger> CRR(P))\<lbrakk>t\<rbrakk>\<^sub>t)"
+  have "\<Phi>(s,\<sigma>,t) wp\<^sub>r CRR(P) = (\<I>(s,t) \<Rightarrow>\<^sub>r (\<lceil>\<sigma>\<rceil>\<^sub>S\<^sub>\<sigma> \<dagger> CRR(P))\<lbrakk>t\<rbrakk>\<^sub>t)"
     by (rel_blast)
   thus ?thesis 
     by (simp add: assms Healthy_if)
 qed
   
-lemma wpR_csp_do_skip [wp]:
+lemma wp_rea_csp_do_skip [wp]:
   fixes Q :: "('\<sigma>, '\<phi>) action"
   assumes "P is CRR"
-  shows "\<Phi>(s,id,t) wp\<^sub>R P = (\<I>(s,t) \<Rightarrow>\<^sub>r P\<lbrakk>t\<rbrakk>\<^sub>t)"
+  shows "\<Phi>(s,id,t) wp\<^sub>r P = (\<I>(s,t) \<Rightarrow>\<^sub>r P\<lbrakk>t\<rbrakk>\<^sub>t)"
 proof -
-  have "\<Phi>(s,id,t) wp\<^sub>R P = \<Phi>(s,id,t) wp\<^sub>R P"
+  have "\<Phi>(s,id,t) wp\<^sub>r P = \<Phi>(s,id,t) wp\<^sub>r P"
     by (simp add: skip_r_def)
   thus ?thesis by (simp add: wp assms usubst alpha)
 qed
@@ -643,7 +643,7 @@ lemma Skip_left_lemma:
   shows "Skip ;; P = \<^bold>R\<^sub>s ((\<forall> $ref \<bullet> pre\<^sub>R P) \<turnstile> (\<exists> $ref \<bullet> cmt\<^sub>R P))"
 proof -
   have "Skip ;; P = 
-        \<^bold>R\<^sub>s (($tr\<acute> =\<^sub>u $tr \<and> $st\<acute> =\<^sub>u $st) wp\<^sub>R pre\<^sub>R P \<turnstile> 
+        \<^bold>R\<^sub>s (($tr\<acute> =\<^sub>u $tr \<and> $st\<acute> =\<^sub>u $st) wp\<^sub>r pre\<^sub>R P \<turnstile> 
             ($tr\<acute> =\<^sub>u $tr \<and> $st\<acute> =\<^sub>u $st) ;; peri\<^sub>R P \<diamondop> 
             ($tr\<acute> =\<^sub>u $tr \<and> $st\<acute> =\<^sub>u $st) ;; post\<^sub>R P)"
     by (simp add: SRD_composition_wp csp_do_def alpha rdes closure wp assms rpred C1, rel_auto)
@@ -734,24 +734,24 @@ lemma CSP3_Continuous: "Continuous CSP3"
 
 lemma Skip_right_lemma:
   assumes "P is CSP"
-  shows "P ;; Skip = \<^bold>R\<^sub>s ((\<not>\<^sub>r pre\<^sub>R P) wp\<^sub>R false \<turnstile> ((\<exists> $st\<acute> \<bullet> cmt\<^sub>R P) \<triangleleft> $wait\<acute> \<triangleright> (\<exists> $ref\<acute> \<bullet> cmt\<^sub>R P)))"
+  shows "P ;; Skip = \<^bold>R\<^sub>s ((\<not>\<^sub>r pre\<^sub>R P) wp\<^sub>r false \<turnstile> ((\<exists> $st\<acute> \<bullet> cmt\<^sub>R P) \<triangleleft> $wait\<acute> \<triangleright> (\<exists> $ref\<acute> \<bullet> cmt\<^sub>R P)))"
 proof -
-  have "P ;; Skip = \<^bold>R\<^sub>s ((\<not>\<^sub>r pre\<^sub>R P) wp\<^sub>R false \<turnstile> (\<exists> $st\<acute> \<bullet> peri\<^sub>R P) \<diamondop> post\<^sub>R P ;; ($tr\<acute> =\<^sub>u $tr \<and> $st\<acute> =\<^sub>u $st))"
+  have "P ;; Skip = \<^bold>R\<^sub>s ((\<not>\<^sub>r pre\<^sub>R P) wp\<^sub>r false \<turnstile> (\<exists> $st\<acute> \<bullet> peri\<^sub>R P) \<diamondop> post\<^sub>R P ;; ($tr\<acute> =\<^sub>u $tr \<and> $st\<acute> =\<^sub>u $st))"
     by (simp add: SRD_composition_wp closure assms wp rdes rpred, rel_auto)
-  also have "... = \<^bold>R\<^sub>s ((\<not>\<^sub>r pre\<^sub>R P) wp\<^sub>R false \<turnstile>
+  also have "... = \<^bold>R\<^sub>s ((\<not>\<^sub>r pre\<^sub>R P) wp\<^sub>r false \<turnstile>
                        ((cmt\<^sub>R P ;; (\<exists> $st \<bullet> \<lceil>II\<rceil>\<^sub>D)) \<triangleleft> $wait\<acute> \<triangleright> (cmt\<^sub>R P ;; ($tr\<acute> =\<^sub>u $tr \<and> \<not> $wait \<and> $st\<acute> =\<^sub>u $st))))"
     by (rule cong[of "\<^bold>R\<^sub>s" "\<^bold>R\<^sub>s"], simp, rel_auto)
-  also have "... = \<^bold>R\<^sub>s ((\<not>\<^sub>r pre\<^sub>R P) wp\<^sub>R false \<turnstile>
+  also have "... = \<^bold>R\<^sub>s ((\<not>\<^sub>r pre\<^sub>R P) wp\<^sub>r false \<turnstile>
                        ((\<exists> $st\<acute> \<bullet> cmt\<^sub>R P) \<triangleleft> $wait\<acute> \<triangleright> (cmt\<^sub>R P ;; ($tr\<acute> =\<^sub>u $tr \<and> \<not> $wait \<and> $st\<acute> =\<^sub>u $st))))"
     by (rule cong[of "\<^bold>R\<^sub>s" "\<^bold>R\<^sub>s"], simp, rel_auto)
-  also have "... = \<^bold>R\<^sub>s ((\<not>\<^sub>r pre\<^sub>R P) wp\<^sub>R false \<turnstile> ((\<exists> $st\<acute> \<bullet> cmt\<^sub>R P) \<triangleleft> $wait\<acute> \<triangleright> (\<exists> $ref\<acute> \<bullet> cmt\<^sub>R P)))"
+  also have "... = \<^bold>R\<^sub>s ((\<not>\<^sub>r pre\<^sub>R P) wp\<^sub>r false \<turnstile> ((\<exists> $st\<acute> \<bullet> cmt\<^sub>R P) \<triangleleft> $wait\<acute> \<triangleright> (\<exists> $ref\<acute> \<bullet> cmt\<^sub>R P)))"
     by (rule cong[of "\<^bold>R\<^sub>s" "\<^bold>R\<^sub>s"], simp, rel_auto)
   finally show ?thesis .
 qed
 
 lemma Skip_right_tri_lemma:
   assumes "P is CSP"
-  shows "P ;; Skip = \<^bold>R\<^sub>s ((\<not>\<^sub>r pre\<^sub>R P) wp\<^sub>R false \<turnstile> ((\<exists> $st\<acute> \<bullet> peri\<^sub>R P) \<diamondop> (\<exists> $ref\<acute> \<bullet> post\<^sub>R P)))"
+  shows "P ;; Skip = \<^bold>R\<^sub>s ((\<not>\<^sub>r pre\<^sub>R P) wp\<^sub>r false \<turnstile> ((\<exists> $st\<acute> \<bullet> peri\<^sub>R P) \<diamondop> (\<exists> $ref\<acute> \<bullet> post\<^sub>R P)))"
 proof -
   have "((\<exists> $st\<acute> \<bullet> cmt\<^sub>R P) \<triangleleft> $wait\<acute> \<triangleright> (\<exists> $ref\<acute> \<bullet> cmt\<^sub>R P)) = ((\<exists> $st\<acute> \<bullet> peri\<^sub>R P) \<diamondop> (\<exists> $ref\<acute> \<bullet> post\<^sub>R P))"
     by (rel_auto)
@@ -763,10 +763,10 @@ lemma CSP4_intro:
           "$st\<acute> \<sharp> (cmt\<^sub>R P)\<lbrakk>true/$wait\<acute>\<rbrakk>" "$ref\<acute> \<sharp> (cmt\<^sub>R P)\<lbrakk>false/$wait\<acute>\<rbrakk>"
   shows "P is CSP4"
 proof -
-  have "CSP4(P) = \<^bold>R\<^sub>s ((\<not>\<^sub>r pre\<^sub>R P) wp\<^sub>R false \<turnstile> ((\<exists> $st\<acute> \<bullet> cmt\<^sub>R P) \<triangleleft> $wait\<acute> \<triangleright> (\<exists> $ref\<acute> \<bullet> cmt\<^sub>R P)))"
+  have "CSP4(P) = \<^bold>R\<^sub>s ((\<not>\<^sub>r pre\<^sub>R P) wp\<^sub>r false \<turnstile> ((\<exists> $st\<acute> \<bullet> cmt\<^sub>R P) \<triangleleft> $wait\<acute> \<triangleright> (\<exists> $ref\<acute> \<bullet> cmt\<^sub>R P)))"
     by (simp add: CSP4_def Skip_right_lemma assms(1))
   also have "... = \<^bold>R\<^sub>s (pre\<^sub>R(P) \<turnstile> ((\<exists> $st\<acute> \<bullet> cmt\<^sub>R P)\<lbrakk>true/$wait\<acute>\<rbrakk> \<triangleleft> $wait\<acute> \<triangleright> (\<exists> $ref\<acute> \<bullet> cmt\<^sub>R P)\<lbrakk>false/$wait\<acute>\<rbrakk>))"
-    by (simp add: wpR_def assms(2) rpred closure cond_var_subst_left cond_var_subst_right)
+    by (simp add: wp_rea_def assms(2) rpred closure cond_var_subst_left cond_var_subst_right)
   also have "... = \<^bold>R\<^sub>s (pre\<^sub>R(P) \<turnstile> ((\<exists> $st\<acute> \<bullet> (cmt\<^sub>R P)\<lbrakk>true/$wait\<acute>\<rbrakk>) \<triangleleft> $wait\<acute> \<triangleright> (\<exists> $ref\<acute> \<bullet> (cmt\<^sub>R P)\<lbrakk>false/$wait\<acute>\<rbrakk>)))"
     by (simp add: usubst unrest)
   also have "... = \<^bold>R\<^sub>s (pre\<^sub>R P \<turnstile> ((cmt\<^sub>R P)\<lbrakk>true/$wait\<acute>\<rbrakk> \<triangleleft> $wait\<acute> \<triangleright> (cmt\<^sub>R P)\<lbrakk>false/$wait\<acute>\<rbrakk>))"
@@ -785,7 +785,7 @@ lemma CSP4_RC_intro:
   shows "P is CSP4"
 proof -
   have "(\<not>\<^sub>r pre\<^sub>R(P)) ;; R1(true) = (\<not>\<^sub>r pre\<^sub>R(P))"
-    by (metis (no_types, lifting) R1_seqr_closure assms(2) rea_not_R1 rea_not_false rea_not_not wpR_RC_false wpR_def)
+    by (metis (no_types, lifting) R1_seqr_closure assms(2) rea_not_R1 rea_not_false rea_not_not wp_rea_RC_false wp_rea_def)
   thus ?thesis
     by (simp add: CSP4_intro assms)
 qed
@@ -886,13 +886,13 @@ lemma CSP4_st'_unrest_peri [unrest]:
 
 lemma CSP4_healthy_form:
   assumes "P is CSP" "P is CSP4"
-  shows "P = \<^bold>R\<^sub>s((\<not>\<^sub>r pre\<^sub>R P) wp\<^sub>R false \<turnstile> ((\<exists> $st\<acute> \<bullet> peri\<^sub>R(P)) \<diamondop> (\<exists> $ref\<acute> \<bullet> post\<^sub>R(P))))"
+  shows "P = \<^bold>R\<^sub>s((\<not>\<^sub>r pre\<^sub>R P) wp\<^sub>r false \<turnstile> ((\<exists> $st\<acute> \<bullet> peri\<^sub>R(P)) \<diamondop> (\<exists> $ref\<acute> \<bullet> post\<^sub>R(P))))"
 proof -
-  have "P = \<^bold>R\<^sub>s ((\<not>\<^sub>r pre\<^sub>R P) wp\<^sub>R false \<turnstile> ((\<exists> $st\<acute> \<bullet> cmt\<^sub>R P) \<triangleleft> $wait\<acute> \<triangleright> (\<exists> $ref\<acute> \<bullet> cmt\<^sub>R P)))"
+  have "P = \<^bold>R\<^sub>s ((\<not>\<^sub>r pre\<^sub>R P) wp\<^sub>r false \<turnstile> ((\<exists> $st\<acute> \<bullet> cmt\<^sub>R P) \<triangleleft> $wait\<acute> \<triangleright> (\<exists> $ref\<acute> \<bullet> cmt\<^sub>R P)))"
     by (metis CSP4_def Healthy_def Skip_right_lemma assms(1) assms(2))
-  also have "... = \<^bold>R\<^sub>s ((\<not>\<^sub>r pre\<^sub>R P) wp\<^sub>R false \<turnstile> ((\<exists> $st\<acute> \<bullet> cmt\<^sub>R P)\<lbrakk>true/$wait\<acute>\<rbrakk> \<triangleleft> $wait\<acute> \<triangleright> (\<exists> $ref\<acute> \<bullet> cmt\<^sub>R P)\<lbrakk>false/$wait\<acute>\<rbrakk>))"
+  also have "... = \<^bold>R\<^sub>s ((\<not>\<^sub>r pre\<^sub>R P) wp\<^sub>r false \<turnstile> ((\<exists> $st\<acute> \<bullet> cmt\<^sub>R P)\<lbrakk>true/$wait\<acute>\<rbrakk> \<triangleleft> $wait\<acute> \<triangleright> (\<exists> $ref\<acute> \<bullet> cmt\<^sub>R P)\<lbrakk>false/$wait\<acute>\<rbrakk>))"
     by (metis (no_types, hide_lams) subst_wait'_left_subst subst_wait'_right_subst wait'_cond_def)
-  also have "... = \<^bold>R\<^sub>s((\<not>\<^sub>r pre\<^sub>R P) wp\<^sub>R false \<turnstile> ((\<exists> $st\<acute> \<bullet> peri\<^sub>R(P)) \<diamondop> (\<exists> $ref\<acute> \<bullet> post\<^sub>R(P))))"
+  also have "... = \<^bold>R\<^sub>s((\<not>\<^sub>r pre\<^sub>R P) wp\<^sub>r false \<turnstile> ((\<exists> $st\<acute> \<bullet> peri\<^sub>R(P)) \<diamondop> (\<exists> $ref\<acute> \<bullet> post\<^sub>R(P))))"
     by (simp add: wait'_cond_def usubst peri\<^sub>R_def post\<^sub>R_def cmt\<^sub>R_def unrest)
   finally show ?thesis .
 qed
@@ -901,13 +901,13 @@ lemma CSP4_ref'_unrest_pre [unrest]:
   assumes "P is CSP" "P is CSP4"
   shows "$ref\<acute> \<sharp> pre\<^sub>R(P)"
 proof -
-  have "pre\<^sub>R(P) = pre\<^sub>R(\<^bold>R\<^sub>s((\<not>\<^sub>r pre\<^sub>R P) wp\<^sub>R false \<turnstile> ((\<exists> $st\<acute> \<bullet> peri\<^sub>R(P)) \<diamondop> (\<exists> $ref\<acute> \<bullet> post\<^sub>R(P)))))"
+  have "pre\<^sub>R(P) = pre\<^sub>R(\<^bold>R\<^sub>s((\<not>\<^sub>r pre\<^sub>R P) wp\<^sub>r false \<turnstile> ((\<exists> $st\<acute> \<bullet> peri\<^sub>R(P)) \<diamondop> (\<exists> $ref\<acute> \<bullet> post\<^sub>R(P)))))"
     using CSP4_healthy_form assms(1) assms(2) by fastforce
-  also have "... = (\<not>\<^sub>r pre\<^sub>R P) wp\<^sub>R false"
-    by (simp add: rea_pre_RHS_design wpR_def usubst unrest
+  also have "... = (\<not>\<^sub>r pre\<^sub>R P) wp\<^sub>r false"
+    by (simp add: rea_pre_RHS_design wp_rea_def usubst unrest
         CSP4_neg_pre_unit R1_rea_not R2c_preR R2c_rea_not assms)
   also have "$ref\<acute> \<sharp> ..."
-    by (simp add: wpR_def unrest)
+    by (simp add: wp_rea_def unrest)
   finally show ?thesis .
 qed
 
@@ -915,12 +915,12 @@ lemma CSP4_ref'_unrest_post [unrest]:
   assumes "P is CSP" "P is CSP4"
   shows "$ref\<acute> \<sharp> post\<^sub>R(P)"
 proof -
-  have "post\<^sub>R(P) = post\<^sub>R(\<^bold>R\<^sub>s((\<not>\<^sub>r pre\<^sub>R P) wp\<^sub>R false \<turnstile> ((\<exists> $st\<acute> \<bullet> peri\<^sub>R(P)) \<diamondop> (\<exists> $ref\<acute> \<bullet> post\<^sub>R(P)))))"
+  have "post\<^sub>R(P) = post\<^sub>R(\<^bold>R\<^sub>s((\<not>\<^sub>r pre\<^sub>R P) wp\<^sub>r false \<turnstile> ((\<exists> $st\<acute> \<bullet> peri\<^sub>R(P)) \<diamondop> (\<exists> $ref\<acute> \<bullet> post\<^sub>R(P)))))"
     using CSP4_healthy_form assms(1) assms(2) by fastforce
-  also have "... = R1 (R2c ((\<not>\<^sub>r pre\<^sub>R P) wp\<^sub>R false \<Rightarrow>\<^sub>r (\<exists> $ref\<acute> \<bullet> post\<^sub>R P)))"
-    by (simp add: rea_post_RHS_design usubst unrest wpR_def)
+  also have "... = R1 (R2c ((\<not>\<^sub>r pre\<^sub>R P) wp\<^sub>r false \<Rightarrow>\<^sub>r (\<exists> $ref\<acute> \<bullet> post\<^sub>R P)))"
+    by (simp add: rea_post_RHS_design usubst unrest wp_rea_def)
   also have "$ref\<acute> \<sharp> ..."
-    by (simp add: R1_def R2c_def wpR_def unrest)
+    by (simp add: R1_def R2c_def wp_rea_def unrest)
   finally show ?thesis .
 qed
 
@@ -1049,7 +1049,7 @@ lemma NCSP_rdes_intro:
   apply (simp_all add: rdes closure assms unrest)
   apply (rule CSP4_tri_intro)
   apply (simp_all add: rdes closure assms unrest)
-  apply (metis (no_types, lifting) CRC_implies_RC R1_seqr_closure assms(1) rea_not_R1 rea_not_false rea_not_not wpR_RC_false wpR_def)
+  apply (metis (no_types, lifting) CRC_implies_RC R1_seqr_closure assms(1) rea_not_R1 rea_not_false rea_not_not wp_rea_RC_false wp_rea_def)
 done
     
 lemma NCSP_preR_CRC [closure]:
@@ -2266,17 +2266,17 @@ lemma "R1((\<not>\<^sub>r P)\<lbrakk>e/&tt\<rbrakk>) = R1(\<not>\<^sub>r P\<lbra
 lemma "R1((P \<Rightarrow>\<^sub>r Q)\<lbrakk>e/&tt\<rbrakk>) = (R1(P\<lbrakk>e/&tt\<rbrakk>) \<Rightarrow>\<^sub>r R1(Q\<lbrakk>e/&tt\<rbrakk>))"
   by (rel_auto)
   
-lemma wpR_DoCSP:
+lemma wp_rea_DoCSP:
   assumes "P is NCSP"
-  shows "($tr\<acute> =\<^sub>u $tr ^\<^sub>u \<langle>\<lceil>a\<rceil>\<^sub>S\<^sub><\<rangle> \<and> $st\<acute> =\<^sub>u $st) wp\<^sub>R pre\<^sub>R P = 
+  shows "($tr\<acute> =\<^sub>u $tr ^\<^sub>u \<langle>\<lceil>a\<rceil>\<^sub>S\<^sub><\<rangle> \<and> $st\<acute> =\<^sub>u $st) wp\<^sub>r pre\<^sub>R P = 
          (\<not>\<^sub>r (\<not>\<^sub>r pre\<^sub>R P)\<lbrakk>$tr ^\<^sub>u \<langle>\<lceil>a\<rceil>\<^sub>S\<^sub><\<rangle>/$tr\<rbrakk>)"
-  by (simp add: wpR_def PrefixCSP_RHS_tri_lemma3 unrest usubst ex_unrest assms closure)    
+  by (simp add: wp_rea_def PrefixCSP_RHS_tri_lemma3 unrest usubst ex_unrest assms closure)    
     
-lemma wpR_DoCSP_alt:
+lemma wp_rea_DoCSP_alt:
   assumes "P is NCSP"
-  shows "($tr\<acute> =\<^sub>u $tr ^\<^sub>u \<langle>\<lceil>a\<rceil>\<^sub>S\<^sub><\<rangle> \<and> $st\<acute> =\<^sub>u $st) wp\<^sub>R pre\<^sub>R P = 
+  shows "($tr\<acute> =\<^sub>u $tr ^\<^sub>u \<langle>\<lceil>a\<rceil>\<^sub>S\<^sub><\<rangle> \<and> $st\<acute> =\<^sub>u $st) wp\<^sub>r pre\<^sub>R P = 
          ($tr\<acute> \<ge>\<^sub>u $tr ^\<^sub>u \<langle>\<lceil>a\<rceil>\<^sub>S\<^sub><\<rangle> \<Rightarrow>\<^sub>r (pre\<^sub>R P)\<lbrakk>$tr ^\<^sub>u \<langle>\<lceil>a\<rceil>\<^sub>S\<^sub><\<rangle>/$tr\<rbrakk>)"  
-  by (simp add: wpR_DoCSP assms rea_not_def R1_def usubst unrest, rel_auto)
+  by (simp add: wp_rea_DoCSP assms rea_not_def R1_def usubst unrest, rel_auto)
           
 lemma trace_ext_R1_closed [closure]: "P is R1 \<Longrightarrow> P\<lbrakk>$tr ^\<^sub>u e/$tr\<rbrakk> is R1"
   by (rel_blast)
@@ -2501,13 +2501,13 @@ lemma GuardedChoiceCSP [rdes_def]:
   by (simp add: PrefixCSP_RHS_tri assms ExtChoice_tri_rdes closure unrest, rel_auto)
 
 (*
-lemma wpR_thing [wp]:
+lemma wp_rea_thing [wp]:
   assumes "\<And> a. P(a) is NCSP"
-  shows "(($tr\<acute> =\<^sub>u $tr ^\<^sub>u \<langle>\<lceil>\<guillemotleft>a\<guillemotright>\<rceil>\<^sub>S\<^sub><\<rangle> \<and> $st\<acute> =\<^sub>u $st) wp\<^sub>R (pre\<^sub>R (P(last\<^sub>u($tr))))) = (pre\<^sub>R(P last\<^sub>u($tr)))\<lbrakk>$tr ^\<^sub>u \<langle>\<lceil>\<guillemotleft>a\<guillemotright>\<rceil>\<^sub>S\<^sub><\<rangle>/$tr\<rbrakk>"
+  shows "(($tr\<acute> =\<^sub>u $tr ^\<^sub>u \<langle>\<lceil>\<guillemotleft>a\<guillemotright>\<rceil>\<^sub>S\<^sub><\<rangle> \<and> $st\<acute> =\<^sub>u $st) wp\<^sub>r (pre\<^sub>R (P(last\<^sub>u($tr))))) = (pre\<^sub>R(P last\<^sub>u($tr)))\<lbrakk>$tr ^\<^sub>u \<langle>\<lceil>\<guillemotleft>a\<guillemotright>\<rceil>\<^sub>S\<^sub><\<rangle>/$tr\<rbrakk>"
   (is "?lhs = ?rhs")
 proof -
   have "?lhs = (\<not> ($tr\<acute> =\<^sub>u $tr ^\<^sub>u \<langle>\<lceil>\<guillemotleft>a\<guillemotright>\<rceil>\<^sub>S\<^sub><\<rangle> \<and> $st\<acute> =\<^sub>u $st) ;; (\<not> pre\<^sub>R (P last\<^sub>u($tr))))"
-    by (simp add: wpR_def R1_neg_preR closure assms)
+    by (simp add: wp_rea_def R1_neg_preR closure assms)
   also have "... = (\<not> ($tr\<acute> =\<^sub>u $tr ^\<^sub>u \<langle>\<lceil>\<guillemotleft>a\<guillemotright>\<rceil>\<^sub>S\<^sub><\<rangle> \<and> $st\<acute> =\<^sub>u $st) ;; (\<exists> $ref \<bullet> (\<not> pre\<^sub>R (P last\<^sub>u($tr)))))"
     by (simp add: ex_unrest unrest assms closure)
   also have "... = (\<not> (\<exists> $ref \<bullet> (\<not> pre\<^sub>R (P last\<^sub>u($tr))))\<lbrakk>$tr ^\<^sub>u \<langle>\<lceil>\<guillemotleft>a\<guillemotright>\<rceil>\<^sub>S\<^sub><\<rangle>/$tr\<rbrakk>)"
@@ -2727,10 +2727,10 @@ lemma Productive_seq_1 [closure]:
 proof -
   have "P ;; Q = \<^bold>R\<^sub>s(pre\<^sub>R(P) \<turnstile> peri\<^sub>R(P) \<diamondop> (post\<^sub>R(P) \<and> $tr <\<^sub>u $tr\<acute>)) ;; \<^bold>R\<^sub>s(pre\<^sub>R(Q) \<turnstile> peri\<^sub>R(Q) \<diamondop> (post\<^sub>R(Q)))"
     by (metis Healthy_def NCSP_implies_CSP SRD_reactive_tri_design Productive_form assms(1) assms(2) assms(3))
-  also have "... = \<^bold>R\<^sub>s ((pre\<^sub>R P \<and> (post\<^sub>R P \<and> $tr\<acute> >\<^sub>u $tr) wp\<^sub>R pre\<^sub>R Q) \<turnstile>
+  also have "... = \<^bold>R\<^sub>s ((pre\<^sub>R P \<and> (post\<^sub>R P \<and> $tr\<acute> >\<^sub>u $tr) wp\<^sub>r pre\<^sub>R Q) \<turnstile>
                        (peri\<^sub>R P \<or> ((post\<^sub>R P \<and> $tr\<acute> >\<^sub>u $tr) ;; peri\<^sub>R Q)) \<diamondop> ((post\<^sub>R P \<and> $tr\<acute> >\<^sub>u $tr) ;; post\<^sub>R Q))"
-    by (simp add: RHS_tri_design_composition_wp rpred unrest closure assms wp NSRD_neg_pre_left_zero  SRD_healths ex_unrest wpR_def disj_upred_def)
-  also have "... = \<^bold>R\<^sub>s ((pre\<^sub>R P \<and> (post\<^sub>R P \<and> $tr\<acute> >\<^sub>u $tr) wp\<^sub>R pre\<^sub>R Q) \<turnstile>
+    by (simp add: RHS_tri_design_composition_wp rpred unrest closure assms wp NSRD_neg_pre_left_zero  SRD_healths ex_unrest wp_rea_def disj_upred_def)
+  also have "... = \<^bold>R\<^sub>s ((pre\<^sub>R P \<and> (post\<^sub>R P \<and> $tr\<acute> >\<^sub>u $tr) wp\<^sub>r pre\<^sub>R Q) \<turnstile>
                        (peri\<^sub>R P \<or> ((post\<^sub>R P \<and> $tr\<acute> >\<^sub>u $tr) ;; peri\<^sub>R Q)) \<diamondop> ((post\<^sub>R P \<and> $tr\<acute> >\<^sub>u $tr) ;; post\<^sub>R Q \<and> $tr\<acute> >\<^sub>u $tr))"
   proof -
     have "((post\<^sub>R P \<and> $tr\<acute> >\<^sub>u $tr) ;; R1(post\<^sub>R Q)) = ((post\<^sub>R P \<and> $tr\<acute> >\<^sub>u $tr) ;; R1(post\<^sub>R Q) \<and> $tr\<acute> >\<^sub>u $tr)"
@@ -2739,7 +2739,7 @@ proof -
       by (simp add: NCSP_implies_NSRD NSRD_is_SRD R1_post_SRD assms)
   qed
   also have "... is Productive"
-    by (rule Productive_rdes_intro, simp_all add: unrest assms closure wpR_def)
+    by (rule Productive_rdes_intro, simp_all add: unrest assms closure wp_rea_def)
   finally show ?thesis .
 qed
 
@@ -2749,9 +2749,9 @@ lemma Productive_seq_2 [closure]:
 proof -
   have "P ;; Q = \<^bold>R\<^sub>s(pre\<^sub>R(P) \<turnstile> peri\<^sub>R(P) \<diamondop> (post\<^sub>R(P))) ;; \<^bold>R\<^sub>s(pre\<^sub>R(Q) \<turnstile> peri\<^sub>R(Q) \<diamondop> (post\<^sub>R(Q) \<and> $tr <\<^sub>u $tr\<acute>))"
     by (metis Healthy_def NCSP_implies_CSP SRD_reactive_tri_design Productive_form assms)
-  also have "... = \<^bold>R\<^sub>s ((pre\<^sub>R P \<and> post\<^sub>R P wp\<^sub>R pre\<^sub>R Q) \<turnstile> (peri\<^sub>R P \<or> (post\<^sub>R P ;; peri\<^sub>R Q)) \<diamondop> (post\<^sub>R P ;; (post\<^sub>R Q \<and> $tr\<acute> >\<^sub>u $tr)))"
-    by (simp add: RHS_tri_design_composition_wp rpred unrest closure assms wp NSRD_neg_pre_left_zero  SRD_healths ex_unrest wpR_def disj_upred_def)
-  also have "... = \<^bold>R\<^sub>s ((pre\<^sub>R P \<and> post\<^sub>R P wp\<^sub>R pre\<^sub>R Q) \<turnstile> (peri\<^sub>R P \<or> (post\<^sub>R P ;; peri\<^sub>R Q)) \<diamondop> (post\<^sub>R P ;; (post\<^sub>R Q \<and> $tr\<acute> >\<^sub>u $tr) \<and> $tr\<acute> >\<^sub>u $tr))"
+  also have "... = \<^bold>R\<^sub>s ((pre\<^sub>R P \<and> post\<^sub>R P wp\<^sub>r pre\<^sub>R Q) \<turnstile> (peri\<^sub>R P \<or> (post\<^sub>R P ;; peri\<^sub>R Q)) \<diamondop> (post\<^sub>R P ;; (post\<^sub>R Q \<and> $tr\<acute> >\<^sub>u $tr)))"
+    by (simp add: RHS_tri_design_composition_wp rpred unrest closure assms wp NSRD_neg_pre_left_zero  SRD_healths ex_unrest wp_rea_def disj_upred_def)
+  also have "... = \<^bold>R\<^sub>s ((pre\<^sub>R P \<and> post\<^sub>R P wp\<^sub>r pre\<^sub>R Q) \<turnstile> (peri\<^sub>R P \<or> (post\<^sub>R P ;; peri\<^sub>R Q)) \<diamondop> (post\<^sub>R P ;; (post\<^sub>R Q \<and> $tr\<acute> >\<^sub>u $tr) \<and> $tr\<acute> >\<^sub>u $tr))"
   proof -
     have "(R1(post\<^sub>R P) ;; (post\<^sub>R Q \<and> $tr\<acute> >\<^sub>u $tr) \<and> $tr\<acute> >\<^sub>u $tr) = (R1(post\<^sub>R P) ;; (post\<^sub>R Q \<and> $tr\<acute> >\<^sub>u $tr))"
       by (rel_auto)
@@ -2759,7 +2759,7 @@ proof -
       by (simp add: NCSP_implies_NSRD NSRD_is_SRD R1_post_SRD assms)
   qed
   also have "... is Productive"
-    by (rule Productive_rdes_intro, simp_all add: unrest assms closure wpR_def)
+    by (rule Productive_rdes_intro, simp_all add: unrest assms closure wp_rea_def)
   finally show ?thesis .
 qed
 
@@ -2867,12 +2867,12 @@ proof -
   have nc2: "(\<box> P\<in>A \<bullet> P ;; Q) = (\<box> P\<in>A \<bullet> NCSP(P) ;; Q)"
     by (rule_tac ExtChoice_cong, simp add: Healthy_if closure assms)
 
-  have p1: "((\<Squnion> P\<in>A \<bullet> pre\<^sub>R P) \<Rightarrow> (\<Sqinter> P\<in>A \<bullet> post\<^sub>R P)) wp\<^sub>R pre\<^sub>R Q =
-            (\<Squnion> P\<in>A \<bullet> post\<^sub>R P wp\<^sub>R pre\<^sub>R Q)" (is "?lhs = ?rhs")
+  have p1: "((\<Squnion> P\<in>A \<bullet> pre\<^sub>R P) \<Rightarrow> (\<Sqinter> P\<in>A \<bullet> post\<^sub>R P)) wp\<^sub>r pre\<^sub>R Q =
+            (\<Squnion> P\<in>A \<bullet> post\<^sub>R P wp\<^sub>r pre\<^sub>R Q)" (is "?lhs = ?rhs")
   proof -
-    have "?lhs = (\<Squnion> P\<in>A \<bullet> (pre\<^sub>R P \<Rightarrow> post\<^sub>R P) wp\<^sub>R pre\<^sub>R Q)"
+    have "?lhs = (\<Squnion> P\<in>A \<bullet> (pre\<^sub>R P \<Rightarrow> post\<^sub>R P) wp\<^sub>r pre\<^sub>R Q)"
       by (simp add: UINF_impl[THEN sym] wp)
-    also have "... = (\<Squnion> P\<in>A \<bullet> post\<^sub>R P wp\<^sub>R pre\<^sub>R Q)"
+    also have "... = (\<Squnion> P\<in>A \<bullet> post\<^sub>R P wp\<^sub>r pre\<^sub>R Q)"
       by (rule USUP_cong, simp add: SRD_post_under_pre closure assms Healthy_if)
     finally show ?thesis .
   qed
@@ -2890,13 +2890,13 @@ proof -
 
   have pre: "pre\<^sub>R((\<box> P\<in>A \<bullet> P) ;; Q) = pre\<^sub>R (\<box> P\<in>A \<bullet> P ;; Q)"
   proof -
-    have "pre\<^sub>R((\<box> P\<in>A \<bullet> P) ;; Q) = ((\<Squnion> P\<in>A \<bullet> pre\<^sub>R P) \<and> ((\<Squnion> P\<in>A \<bullet> pre\<^sub>R P) \<Rightarrow> (\<Sqinter> P\<in>A \<bullet> post\<^sub>R P)) wp\<^sub>R pre\<^sub>R Q)"
+    have "pre\<^sub>R((\<box> P\<in>A \<bullet> P) ;; Q) = ((\<Squnion> P\<in>A \<bullet> pre\<^sub>R P) \<and> ((\<Squnion> P\<in>A \<bullet> pre\<^sub>R P) \<Rightarrow> (\<Sqinter> P\<in>A \<bullet> post\<^sub>R P)) wp\<^sub>r pre\<^sub>R Q)"
       by (simp add: rdes closure assms wp)
-    also have "... = ((\<Squnion> P\<in>A \<bullet> pre\<^sub>R P) \<and> (\<Squnion> P\<in>A \<bullet> post\<^sub>R P wp\<^sub>R pre\<^sub>R Q))"
+    also have "... = ((\<Squnion> P\<in>A \<bullet> pre\<^sub>R P) \<and> (\<Squnion> P\<in>A \<bullet> post\<^sub>R P wp\<^sub>r pre\<^sub>R Q))"
       by (simp add: p1)
-    also have "... = (\<Squnion> P\<in>A \<bullet> (pre\<^sub>R P \<and> (post\<^sub>R P wp\<^sub>R pre\<^sub>R Q)))"
+    also have "... = (\<Squnion> P\<in>A \<bullet> (pre\<^sub>R P \<and> (post\<^sub>R P wp\<^sub>r pre\<^sub>R Q)))"
       by (rel_blast)
-    also have "... = (\<Squnion> P\<in>A \<bullet> pre\<^sub>R (NCSP P) \<and> post\<^sub>R (NCSP P) wp\<^sub>R pre\<^sub>R Q)"
+    also have "... = (\<Squnion> P\<in>A \<bullet> pre\<^sub>R (NCSP P) \<and> post\<^sub>R (NCSP P) wp\<^sub>r pre\<^sub>R Q)"
       by (rule USUP_cong, simp add: closure assms Healthy_if)
     also have "... = pre\<^sub>R (\<box> P\<in>A \<bullet> P ;; Q)"
       by (simp add: rdes closure assms nc2)
@@ -2906,34 +2906,34 @@ proof -
   have peri: "peri\<^sub>R((\<box> P\<in>A \<bullet> P) ;; Q) = peri\<^sub>R (\<box> P\<in>A \<bullet> P ;; Q)" (is "?lhs = ?rhs")
     apply (simp_all add: rdes nc2 closure assms p1 spec_cond_dist)
   proof -
-    have "?rhs = ((\<Squnion> P\<in>A \<bullet> pre\<^sub>R P \<and> post\<^sub>R P wp\<^sub>R pre\<^sub>R Q) \<Rightarrow>
-                  (\<Squnion> P\<in>A \<bullet> pre\<^sub>R P \<and> post\<^sub>R P wp\<^sub>R pre\<^sub>R Q \<Rightarrow> peri\<^sub>R P \<or> post\<^sub>R P ;; peri\<^sub>R Q)) \<triangleleft> $tr\<acute> =\<^sub>u $tr \<triangleright>
-                  ((\<Squnion> P\<in>A \<bullet> pre\<^sub>R P \<and> post\<^sub>R P wp\<^sub>R pre\<^sub>R Q) \<Rightarrow>
-                   (\<Sqinter> P\<in>A \<bullet> pre\<^sub>R P \<and> post\<^sub>R P wp\<^sub>R pre\<^sub>R Q \<Rightarrow> peri\<^sub>R P \<or> post\<^sub>R P ;; peri\<^sub>R Q))"
+    have "?rhs = ((\<Squnion> P\<in>A \<bullet> pre\<^sub>R P \<and> post\<^sub>R P wp\<^sub>r pre\<^sub>R Q) \<Rightarrow>
+                  (\<Squnion> P\<in>A \<bullet> pre\<^sub>R P \<and> post\<^sub>R P wp\<^sub>r pre\<^sub>R Q \<Rightarrow> peri\<^sub>R P \<or> post\<^sub>R P ;; peri\<^sub>R Q)) \<triangleleft> $tr\<acute> =\<^sub>u $tr \<triangleright>
+                  ((\<Squnion> P\<in>A \<bullet> pre\<^sub>R P \<and> post\<^sub>R P wp\<^sub>r pre\<^sub>R Q) \<Rightarrow>
+                   (\<Sqinter> P\<in>A \<bullet> pre\<^sub>R P \<and> post\<^sub>R P wp\<^sub>r pre\<^sub>R Q \<Rightarrow> peri\<^sub>R P \<or> post\<^sub>R P ;; peri\<^sub>R Q))"
         apply (simp_all add: rdes nc2 closure assms p1 spec_cond_dist unrest)
         apply (subst USUP_healthy[of "A" "NCSP", THEN sym], simp add: assms)+
         apply (subst UINF_healthy[of "A" "NCSP", THEN sym], simp add: assms)+
         apply (simp)
     done
     also
-    have "... = ((\<Squnion> P\<in>A \<bullet> pre\<^sub>R P \<and> post\<^sub>R P wp\<^sub>R pre\<^sub>R Q) \<Rightarrow>
+    have "... = ((\<Squnion> P\<in>A \<bullet> pre\<^sub>R P \<and> post\<^sub>R P wp\<^sub>r pre\<^sub>R Q) \<Rightarrow>
                   (\<Squnion> P\<in>A \<bullet> peri\<^sub>R P \<or> post\<^sub>R P ;; peri\<^sub>R Q)) \<triangleleft> $tr\<acute> =\<^sub>u $tr \<triangleright>
-                  ((\<Squnion> P\<in>A \<bullet> pre\<^sub>R P \<and> post\<^sub>R P wp\<^sub>R pre\<^sub>R Q) \<Rightarrow>
+                  ((\<Squnion> P\<in>A \<bullet> pre\<^sub>R P \<and> post\<^sub>R P wp\<^sub>r pre\<^sub>R Q) \<Rightarrow>
                    (\<Sqinter> P\<in>A \<bullet> peri\<^sub>R P \<or> post\<^sub>R P ;; peri\<^sub>R Q))"
       by (rel_blast)
-    also have "... = ((\<Squnion> P\<in>A \<bullet> pre\<^sub>R P \<and> post\<^sub>R P wp\<^sub>R pre\<^sub>R Q) \<Rightarrow>
+    also have "... = ((\<Squnion> P\<in>A \<bullet> pre\<^sub>R P \<and> post\<^sub>R P wp\<^sub>r pre\<^sub>R Q) \<Rightarrow>
                       (\<Squnion> P\<in>A \<bullet> peri\<^sub>R P \<or> post\<^sub>R P ;; peri\<^sub>R Q) \<triangleleft> $tr\<acute> =\<^sub>u $tr \<triangleright>
                       (\<Sqinter> P\<in>A \<bullet> peri\<^sub>R P \<or> post\<^sub>R P ;; peri\<^sub>R Q))"
       by (simp add: spec_cond_dist[THEN sym] UINF_conj_UINF)
-    also have "... = ((\<Squnion> P\<in>A \<bullet> pre\<^sub>R P \<and> post\<^sub>R P wp\<^sub>R pre\<^sub>R Q) \<Rightarrow>
+    also have "... = ((\<Squnion> P\<in>A \<bullet> pre\<^sub>R P \<and> post\<^sub>R P wp\<^sub>r pre\<^sub>R Q) \<Rightarrow>
                       (\<Squnion> P\<in>A \<bullet> peri\<^sub>R P \<or> pre\<^sub>R P \<and> (post\<^sub>R P ;; peri\<^sub>R Q)) \<triangleleft> $tr\<acute> =\<^sub>u $tr \<triangleright>
                       (\<Sqinter> P\<in>A \<bullet> peri\<^sub>R P \<or> post\<^sub>R P ;; peri\<^sub>R Q))"
       by (rel_auto)
-    also have "... = ((\<Squnion> P\<in>A \<bullet> pre\<^sub>R P \<and> post\<^sub>R P wp\<^sub>R pre\<^sub>R Q) \<Rightarrow>
+    also have "... = ((\<Squnion> P\<in>A \<bullet> pre\<^sub>R P \<and> post\<^sub>R P wp\<^sub>r pre\<^sub>R Q) \<Rightarrow>
                       (\<Squnion> P\<in>A \<bullet> peri\<^sub>R P \<or> pre\<^sub>R P \<and> ((post\<^sub>R P \<and> $tr <\<^sub>u $tr\<acute>) ;; peri\<^sub>R Q)) \<triangleleft> $tr\<acute> =\<^sub>u $tr \<triangleright>
                       (\<Sqinter> P\<in>A \<bullet> peri\<^sub>R P \<or> post\<^sub>R P ;; peri\<^sub>R Q))"
       oops
-    also have "... = ((\<Squnion> P\<in>A \<bullet> pre\<^sub>R P) \<and> (\<Squnion> P\<in>A \<bullet> post\<^sub>R P wp\<^sub>R pre\<^sub>R Q) \<Rightarrow>
+    also have "... = ((\<Squnion> P\<in>A \<bullet> pre\<^sub>R P) \<and> (\<Squnion> P\<in>A \<bullet> post\<^sub>R P wp\<^sub>r pre\<^sub>R Q) \<Rightarrow>
                   ((\<Squnion> P\<in>A \<bullet> peri\<^sub>R P) \<triangleleft> $tr\<acute> =\<^sub>u $tr \<triangleright> (\<Sqinter> P\<in>A \<bullet> peri\<^sub>R P)) \<or>
                   ((\<Sqinter> P\<in>A \<bullet> post\<^sub>R P) ;; peri\<^sub>R Q))"
       apply (rel_simp, safe)
@@ -2942,12 +2942,12 @@ proof -
 
 
 
-    have "?lhs = ((\<Squnion> P\<in>A \<bullet> pre\<^sub>R P) \<and> (\<Squnion> P\<in>A \<bullet> post\<^sub>R P wp\<^sub>R pre\<^sub>R Q) \<Rightarrow>
+    have "?lhs = ((\<Squnion> P\<in>A \<bullet> pre\<^sub>R P) \<and> (\<Squnion> P\<in>A \<bullet> post\<^sub>R P wp\<^sub>r pre\<^sub>R Q) \<Rightarrow>
                   ((\<Squnion> P\<in>A \<bullet> peri\<^sub>R P) \<triangleleft> $tr\<acute> =\<^sub>u $tr \<triangleright> (\<Sqinter> P\<in>A \<bullet> peri\<^sub>R P)) \<or>
                   ((\<Sqinter> P\<in>A \<bullet> post\<^sub>R P) ;; peri\<^sub>R Q))"
       by (simp_all add: rdes nc2 closure assms p1 spec_cond_dist, simp add: p2, rel_auto)
     (*
-"     ((\<Squnion> P\<in>A \<bullet> pre\<^sub>R P) \<and> (\<Squnion> P\<in>A \<bullet> post\<^sub>R P wp\<^sub>R pre\<^sub>R Q) \<Rightarrow>
+"     ((\<Squnion> P\<in>A \<bullet> pre\<^sub>R P) \<and> (\<Squnion> P\<in>A \<bullet> post\<^sub>R P wp\<^sub>r pre\<^sub>R Q) \<Rightarrow>
      ((\<Squnion> P\<in>A \<bullet> peri\<^sub>R P) \<triangleleft> $tr\<acute> =\<^sub>u $tr \<triangleright> (\<Sqinter> P\<in>A \<bullet> peri\<^sub>R P)) \<or>
      ((\<Sqinter> P\<in>A \<bullet> post\<^sub>R P)) ;; peri\<^sub>R Q)" *)
 
@@ -4365,10 +4365,10 @@ lift_definition postC :: "('s, 'e) action \<Rightarrow> ('s, 'e) crel" ("post\<^
   by (simp_all add: unrest closure, rel_auto)
 
 lift_definition wpC :: "('s, 'e) crel \<Rightarrow> ('s, 'e) crel \<Rightarrow> ('s, 'e) crel" (infix "wp\<^sub>C" 60) is "wpR"
-  by (auto simp add: unrest closure SRD_healths wpR_def)
+  by (auto simp add: unrest closure SRD_healths wp_rea_def)
     
 lift_definition rdes :: "('s, 'e) crel \<Rightarrow> ('s, 'e) crel \<Rightarrow> ('s, 'e) crel \<Rightarrow> ('s, 'e) action" is
-"\<lambda> P Q R. \<^bold>R\<^sub>s(P wp\<^sub>R false \<turnstile> (Q ;; ($tr\<acute> =\<^sub>u $tr \<and> $\<Sigma>\<^sub>S\<acute> =\<^sub>u $\<Sigma>\<^sub>S)) \<diamondop> R)" .
+"\<lambda> P Q R. \<^bold>R\<^sub>s(P wp\<^sub>r false \<turnstile> (Q ;; ($tr\<acute> =\<^sub>u $tr \<and> $\<Sigma>\<^sub>S\<acute> =\<^sub>u $\<Sigma>\<^sub>S)) \<diamondop> R)" .
     
 lemma R2_implies_R2c [closure]: "P is R2 \<Longrightarrow> P is R2c"
   by (rel_blast)
@@ -4391,7 +4391,7 @@ lemma rdes_NSRD [closure]: "rdes P Q R is NSRD"
   apply (transfer, auto)
   apply (rule NSRD_intro)
   apply (rule RHS_tri_design_is_SRD)
-  apply (simp_all add: wpR_def rea_pre_RHS_design rea_peri_RHS_design seqr_assoc[THEN sym] usubst 
+  apply (simp_all add: wp_rea_def rea_pre_RHS_design rea_peri_RHS_design seqr_assoc[THEN sym] usubst 
          R2c_true R1_R2c_seqr_distribute R1_rea_not' R2c_rea_not R2c_rea_impl R1_rea_impl' rpred 
          closure unrest)
 done
@@ -4434,17 +4434,17 @@ lemma preC_skip [rdes]: "pre\<^sub>C(Skip) = true"
 lemma periC_skip [rdes]: "peri\<^sub>C(Skip) = false"
   by (simp add: rdes rrel_lift closure)
     
-lemma wpR_R2_closed [closure]: 
-  "\<lbrakk> P is R2; Q is R2 \<rbrakk> \<Longrightarrow> P wp\<^sub>R Q is R2"
-  by (simp add: wpR_def closure)
+lemma wp_rea_R2_closed [closure]: 
+  "\<lbrakk> P is R2; Q is R2 \<rbrakk> \<Longrightarrow> P wp\<^sub>r Q is R2"
+  by (simp add: wp_rea_def closure)
 
-lemma unrest_wpR_1 [unrest]:
-  "\<lbrakk> x \<bowtie> tr; $x \<sharp> P \<rbrakk> \<Longrightarrow> $x \<sharp> P wp\<^sub>R Q"
-  by (simp add: wpR_def unrest)
+lemma unrest_wp_rea_1 [unrest]:
+  "\<lbrakk> x \<bowtie> tr; $x \<sharp> P \<rbrakk> \<Longrightarrow> $x \<sharp> P wp\<^sub>r Q"
+  by (simp add: wp_rea_def unrest)
 
-lemma unrest_wpR_2 [unrest]:
-  "\<lbrakk> x \<bowtie> tr; $x\<acute> \<sharp> Q \<rbrakk> \<Longrightarrow> $x\<acute> \<sharp> P wp\<^sub>R Q"
-  by (simp add: wpR_def unrest)
+lemma unrest_wp_rea_2 [unrest]:
+  "\<lbrakk> x \<bowtie> tr; $x\<acute> \<sharp> Q \<rbrakk> \<Longrightarrow> $x\<acute> \<sharp> P wp\<^sub>r Q"
+  by (simp add: wp_rea_def unrest)
     
 lemma preC_seq [rdes]:
   "\<lbrakk> P is NSRD; Q is NSRD \<rbrakk> \<Longrightarrow> pre\<^sub>C(P ;; Q) = (pre\<^sub>C P \<and> post\<^sub>C P wp\<^sub>C pre\<^sub>C Q)"
